theories/Syntax.v
@@ -1,77 +1,89 @@
-Require Import PeanoNat.
-Require Import Arith.
-From Coq Require Import Unicode.Utf8.
+From Coq Require Import Unicode.Utf8_core.
+From TLC Require Import LibLN LibTactics LibFset.
+From TTSB Require Import Tactics.
 
-Inductive term :Set :=
-  | Trm_Bound_Var : nat -> term
-  | Trm_App : term -> term -> term
-  | Trm_Abs : term -> term 
+
+
+Inductive term := 
+  | TmBVar : nat -> term 
+  | TmFVar : var -> term 
+  | TmAbs : term -> term 
+  | TmApp : term -> term -> term 
 .
 
-Declare Custom Entry term.
-Notation "<{ e }>" := e (e custom term at level 99).
-Notation "( x )" := x (in custom term, x at level 99).
-Notation "x" := x (in custom term at level 0, x constr at level 0).
-Notation "'#' n" := (Trm_Bound_Var n) (in custom term at level 0).
-Notation "x y" := (Trm_App x y) (in custom term at level 2, left associativity).
-Notation "'λ' t" := (Trm_Abs t) (
-  in custom term at level 90, 
-  t custom term at level 99,
-  left associativity
-).
-Notation "'`' e '`'" := e (in custom term at level 0, e constr).
-
-Check <{ (λ #0 #1)(λ #1 #0) }>.
-
-
-Check le_gt_dec.
-Fixpoint shift (n : nat) (k : nat) (t : term) : term := 
+Reserved Notation "{ k ~> u } t" (at level 67).
+Fixpoint open' (k : nat) (u : term) (t : term) : term :=
   match t with 
-  | <{ #p }> => 
-    match le_gt_dec p k with 
-    | left p_le_k => t
-    | right p_gt_k => <{ #`p + n - 1 ` }>
-    end
-  | <{ u v }> => <{`shift n k u` `shift n k v`}> 
-  | <{ λ u }> => <{ λ `shift n (k + 1) u` }>
-  end.
-
-Check lt_eq_lt_dec. 
-Reserved Notation "M '[' n '<-' N ']'" (
-  in custom term at level 0,
-  n constr
-).
-Fixpoint subst (t : term) (n : nat) (s : term) : term := 
-  match t with 
-  | <{ #m }> => 
-    match Nat.eq_dec n m with 
-    | left eq => shift n 0 s
-    | right neq => t
-    end
-  | <{ u v }> => <{(u[n <- s]) (v[n <- s])}>
-  | <{ λ u }> => <{λ u[n+1 <- s]}>
+  | TmBVar i => If i = k then u else t 
+  | TmFVar y => t
+  | TmAbs t' => TmAbs ({ (S k) ~> u } t')
+  | TmApp t1 t2 => TmApp ({k ~> u} t1) (({k ~> u} t2))
   end
-  where
-  "M '[' n '<-' N ']'" := (subst M n N) (in custom term).
+  where 
+  "{ k ~> u } t" := (open' k u t)
+  .
+Definition open : term -> term -> term := open' 0.
+Notation " t ^^ u " := (open u t) (at level 67).
+Notation " t ^ x " := (open (TmFVar x) t).
 
-Fixpoint lower (n : nat) (t : term) : term := 
+Fixpoint fv (t : term) : vars :=
   match t with 
-  | <{#m}> =>
-    match le_gt_dec m n with 
-    | left m_le_n => t
-    | right m_gt_n => <{#`m-1`}>
-    end
-  | <{λ t}> => <{ λ `lower (n+1) t` }>
-  | <{t u}> => <{ `lower n t` `lower n u`}>
+  | TmBVar _ => \{}
+  | TmFVar x => \{x}
+  | TmAbs t' => fv t'
+  | TmApp t1 t2 => fv t1 \u fv t2
   end.
 
-Compute <{ (λ #2 #0 #1)[0 <- #4] }>.
+Inductive lc : term -> Prop :=
+  | LCFVar : 
+      ∀ (x : var), 
+      lc (TmFVar x) 
+  | LCAbs : 
+      ∀ (t : term), 
+      (∀ (x : var), (x \notin fv t) -> lc (t ^ x)) -> 
+      lc (TmAbs t)
+  | LCApp : 
+      ∀ (t1 t2 : term),
+      lc t1 -> lc t2 ->
+      lc (TmApp t1 t2)
+.
 
 
-Notation "t '[' s ']'" := (subst s t) (in custom term at level 1, s at level 99, no associativity).
 
-Check <{ λ λ ((λ #2 #1 #0) (λ #0))  }>.
+Reserved Notation "[ x ~> u ] t" (at level 67).
+Fixpoint subst (x : var) (u : term) (t : term) : term := 
+  match t with 
+  | TmBVar i => t
+  | TmFVar y => If x = y then u else t
+  | TmAbs t' => TmAbs ([x ~> u] t')
+  | TmApp t1 t2 => TmApp ([x ~> u] t1) ([x ~> u] t2)
+  end
+  where "[ x ~> u ] t" := (subst x u t)
+  .
 
-Compute <{(λ λ ((#2 #1 #0) [0 <- λ #0]))}>.
-Eval compute in <{(λ λ ((#2 #1 #0)[1 <- λ #0]))}>.
-Eval compute in <{(λ λ ((#2 #1 #0)))[0 <- λ #0]}>.
+
+Lemma open_eq :
+  ∀ (x : var) (t₁ t₂ : term), 
+  x \notin fv t₁ \u fv t₂ -> 
+  t₁ ^ x = t₂ ^ x -> 
+  t₁ = t₂.
+Proof.
+  unfold "^".
+  generalize 0.
+  introv.
+  inductions t₁ gen n; introv Hnotin Heq; 
+  destruct t₂; unfold "^" in *; simpls*; try solve [inverts Heq];
+  repeat case_if*; substs*; inverts Heq; 
+  repeat (simpl_unions; split_and_or_max); autos*; fequals*.
+Qed.
+
+Lemma open_subst :
+  ∀ t u x,
+  x \notin fv t -> 
+  t ^^ u = [x ~> u](t ^ x). 
+Proof.
+  unfold "^^", "^".
+  generalize 0.
+  intros n t; gen n.
+  induction* t; introv Hnotin; repeat (simpls || reduce_max || case_if); fequals*.
+Qed.
