theories/Types/Context.v
@@ -1,1 +1,394 @@
-Require Import Types.Types.
+From TLC Require Import LibLN LibTactics LibFset.
+From Coq Require Import Unicode.Utf8_core.
+From Coq Require Import Lia.
+From TTSB Require Import Tactics.
+From TTSB Require Import Classes.
+From TTSB.Types Require Types.
+Import Types.TypesNotations.
+Create HintDb context_hints.
+
+Local Notation "'multitype'" := Types.multitype.
+Local Notation "'eq_multitype'" := Types.eq_multitype.
+
+Definition ctx : Type := vars * (var -> multitype).
+Definition empty : ctx := (\{}, fun _ => {{nil}}).
+Definition add (Γ : ctx) (v : var) (e : multitype) : ctx :=
+  If e = {{nil}} 
+  then Γ 
+  else
+    let (s, f) := Γ in 
+    (s \u \{v}, fun x => If x = v then e ⊎ (f x) else f x).
+
+Lemma add_nil :
+  ∀ Γ x, add Γ x {{nil}} = Γ.
+Proof.
+  unfolds add; case_if; reflexivity.
+Qed.
+
+Definition get (Γ : ctx) (x : var) := 
+  let (_, f) := Γ in f x.
+
+
+
+Lemma get_empty :
+  ∀ x, get empty x = {{nil}}.
+Proof.
+  reflexivity.
+Qed.
+
+Lemma get_add_eq : 
+  ∀ Γ x A, get (add Γ x A) x = A ⊎ (get Γ x).
+Proof.
+  unfolds get, add; destruct Γ; intros;
+  repeat case_if; substs*.
+Qed.
+
+Lemma get_add_neq :
+  ∀ Γ x x' A, x ≠ x' -> get (add Γ x A) x' = get Γ x'.
+Proof.
+  unfolds get, add; destruct Γ; intros;
+  repeat case_if; substs*.
+Qed.
+
+
+
+Definition union (Γ₁ Γ₂ : ctx) : ctx :=
+  let (s₁, f₁) := Γ₁ in
+  let (s₂, f₂) := Γ₂ in
+  (s₁ \u s₂, fun x => (f₁ x) ⊎ (f₂ x)).
+
+Notation "a '⊎c' b"  := (union a b) (at level 0).
+
+
+Lemma get_union :
+  ∀ Γ₁ Γ₂ x, 
+  get (Γ₁ ⊎c Γ₂) x = (get Γ₁ x) ⊎ (get Γ₂ x).
+Proof.
+  intros.
+  destruct Γ₁ as [s₁ f₁]. destruct Γ₂ as [s₂ f₂].
+  simpls*.
+Qed.
+Definition equals (Γ₁ Γ₂ : ctx) : Prop :=
+  let (s₁, f₁) := Γ₁ in
+  let (s₂, f₂) := Γ₂ in
+  s₁ = s₂ /\ 
+  ∀ (x : var),  
+  eq_multitype (f₁ x) (f₂ x).
+
+Instance Equiv_equals_ctx : Equivalence equals.
+Proof.
+  use_equivalences.
+  constructor;
+  intros;
+  repeat match goal with 
+  | [ Γ : ctx |- _] => destruct Γ
+  end; simpls; split_and_or_max; substs*.
+Qed.
+
+
+Ltac use_equivalences ::= 
+  Types.use_equivalences_type;
+  destruct Equiv_equals_ctx 
+    as [eq_ctx_refl eq_ctx_sym eq_ctx_trans].
+
+
+Lemma equals_empty_is_empty :
+  ∀ Γ, equals Γ empty <-> Γ = empty.
+Proof.
+  destruct Γ; split; intros; inverts* H.
+  - fequals*. applys fun_ext_dep.
+    intro x.
+    specialize H1 with x.
+    applys* Types.eq_empty_is_empty.
+  - use_equivalences. autos*.
+Qed. 
+
+Lemma equals_add :
+  ∀ Γ₁ Γ₂ x M₁ M₂, 
+  Types.eq_multitype M₁ M₂ ->
+  equals Γ₁ Γ₂ -> 
+  equals (add Γ₁ x M₁) (add Γ₂ x M₂).
+Proof.
+  intros [s1 f1] [s2 f2] * HeqM HeqΓ.
+  unfold add; repeat case_if; substs*;
+  try solve[use_equivalences; hint Types.eq_empty_is_empty; false*].
+  simpls; reduce_max; substs*.
+  hint Types.union_perm.
+  intros.
+  case_if*.
+Qed.
+
+Lemma add_comm :
+  ∀ Γ₁ Γ₂ x₁ x₂ M₁ M₂, 
+  equals Γ₁ Γ₂ -> 
+  equals (add (add Γ₁ x₁ M₁) x₂ M₂) (add (add Γ₂ x₂ M₂) x₁ M₁).
+Proof.
+  intros [s₁ f₁] [s₂ f₂] * Heq.
+  simpls.
+  unfolds add, equals;
+  repeat case_if; reduce_max; substs*;
+  try solve [intro y; hint Types.union_perm; use_equivalences; case_if*]. 
+  - rewrite union_comm, union_assoc, (union_comm \{ x₂} s₂). auto.
+  - intro. repeat case_if; 
+    try solve[ hint Types.union_perm; use_equivalences; autos* ].
+    use_equivalences.
+    hint Types.union_assoc, Types.union_perm, Types.union_comm; autos*.
+Qed.  
+
+
+Lemma union_empty_l :
+  ∀ Γ, (empty ⊎c Γ) = Γ.
+Proof.
+  use_equivalences;
+  intros [s f].
+  simpls.
+  simpl_unions.
+  fequals.
+Qed.
+
+Lemma union_empty_r :
+  ∀ Γ, (Γ ⊎c empty) = Γ.
+Proof.
+  
+  use_equivalences;
+  intros [s f].
+  simpls.
+  simpl_unions.
+  fequals.
+  apply fun_ext_dep; intro.
+  rewrite* Types.union_empty_r.
+Qed.
+
+Lemma union_comm :
+  ∀ Γ₁ Γ₂, equals (Γ₁ ⊎c Γ₂) (Γ₂ ⊎c Γ₁).
+Proof.
+  hint Types.union_comm.
+  intros [s₁ f₁] [s₂ f₂]; simpls*; splits*;
+  apply* LibFset.union_comm.
+Qed.
+
+Lemma union_assoc :
+  ∀ Γ₁ Γ₂ Γ₃, equals ((Γ₁ ⊎c Γ₂) ⊎c Γ₃) (Γ₁ ⊎c (Γ₂ ⊎c Γ₃)).
+Proof.
+  hint Types.union_assoc.
+  intros [s₁ f₁] [s₂ f₂] [s₃ f₃]; simpls*; splits*.
+  rewrite* LibFset.union_assoc.
+Qed.
+
+Definition ok (Γ : ctx) : Prop := 
+  let (s, f) := Γ in 
+  ∀ x, x \in s <-> f x ≠ {{nil}}.
+
+
+Lemma ok_empty :
+  ok empty.
+Proof.
+  unfolds empty. simpls.
+  intros; splits; intro H_contra; false.
+  applys* in_empty_inv.
+Qed.
+Hint Resolve ok_empty : context_hints.
+
+
+Lemma ok_add : 
+  ∀ (Γ : ctx) (x : var) (M : multitype),
+    ok Γ -> 
+    ok (add Γ x M).
+Proof.
+  intros [s f] y M Hok.
+  unfolds ok, add; repeat case_if; intro x; specialize Hok with x; split_and_or_max; intros; repeat case_if*; autos*.
+  - applys* Types.nnil_union.
+  - apply Hok0; reduce_max; autos*.
+  - reduce_max; right; reduce_max; autos.
+  - simpl_unions; autos*.
+Qed. 
+
+
+Lemma ok_union :
+  ∀ (Γ₁ Γ₂ : ctx),
+  ok Γ₁ -> ok Γ₂ ->
+  ok Γ₁ ⊎c Γ₂.
+Proof.
+  hint Types.nnil_union.
+  unfolds ok, union.
+  intros [s₁ f₁] [s₂ f₂] Hok1 Hok2 x.
+  specialize Hok1 with x;
+  specialize Hok2 with x;
+  split_and_or_max; intros; repeat simpl_unions.
+  - applys* Types.nnil_union.
+  - destruct (f₁ x); destruct (f₂ x); autos*;
+    left; applys Hok4; absurd.
+Qed.
+
+Lemma ok_eq : 
+  ∀ Γ₁ Γ₂, 
+  equals Γ₁ Γ₂ ->
+  ok Γ₁ ->
+  ok Γ₂.
+Proof.
+  hint Types.eq_empty_is_empty.
+  use_equivalences.
+  intros [s₁ f₁] [s₂ f₂] [H_eq_dom H_eq_f] Hok; simpls*.
+  intro x.
+  specialize Hok with x as [H_in_nnil H_nnil_in].
+  specialize H_eq_f with x; substs; split_and_or_max.
+  - intros Hin H_contra.
+    applys* H_in_nnil.
+    rewrites* H_contra in H_eq_f.
+  - intros H_f2x_nnil.
+    apply H_nnil_in.
+    destruct (f₁ x); destruct* (f₂ x).
+    absurd.
+Qed.
+
+Lemma add_eq: 
+  ∀ x M Γ₁ Γ₂,
+  ok Γ₁ -> ok Γ₂ ->
+  equals (add Γ₁ x M) (add Γ₂ x M) -> 
+  equals Γ₁ Γ₂.
+Proof.
+  intros x M [s₁ f₁] [s₂ f₂] Hok1 Hok2 Heq; unfolds equals, add; case_if; simpls; split_and_or_max; autos.
+  - lets Heq2 : Heq1 x; case_if.
+    destruct (f₁ x) eqn:Heqf₁x;
+    destruct (f₂ x) eqn:Heqf₂x;
+    try rewrite Types.union_empty_r in Heq2;
+    try solve[
+      apply Types.eq_size in Heq2; rewrite Types.size_union in Heq2; 
+      simpls; lia
+    ].
+    + admit.
+    + admit.
+  - lets Heq2 : Heq1 x; case_if.
+    destruct (f₁ x) eqn:Heqf₁x;
+    destruct (f₂ x) eqn:Heqf₂x;
+    try rewrite Types.union_empty_r in Heq2; 
+    try solve[
+      apply Types.eq_size in Heq2; rewrite Types.size_union in Heq2; 
+      simpls; lia
+    ].
+    + intro y.
+      asserts H_EM : ({x = y} + {¬ x = y}).
+      { apply classicT. }
+      destruct H_EM.
+      * substs; use_equivalences; rewrite Heqf₁x, Heqf₂x; autos*.
+      * substs; specialize Heq1 with y; case_if*.
+    + intro y.
+      asserts H_EM : ({x = y} + {¬ x = y}).
+      { apply classicT. }
+      destruct H_EM.
+      * substs; use_equivalences; rewrite Heqf₁x, Heqf₂x; autos*. admit.
+      * substs; specialize Heq1 with y; case_if*.
+Admitted.
+
+
+Definition dom (Γ₁ : ctx) : vars := fst Γ₁.
+
+Lemma dom_add : 
+  ∀ Γ x mt,
+  mt ≠ {{nil}} ->
+  dom (add Γ x mt) = \{x} \u (dom Γ).
+Proof.
+  intros.
+  destruct Γ eqn:HeqΓ.
+  destruct (add (v, m) x mt) eqn:HeqAdd.
+  simpl.
+  unfold add in *.
+  case_if*.
+  inverts HeqAdd.
+  rewrite* LibFset.union_comm.
+Qed.
+
+Lemma dom_union :
+  ∀ Γ₁ Γ₂,
+  dom (Γ₁ ⊎c Γ₂) = (dom Γ₁) \u (dom Γ₂).
+Proof.
+  intros [s₁ f₁] [s₂ f₂].
+  simpls*.
+Qed.
+
+Lemma dom_equal :
+  ∀ Γ₁ Γ₂,
+  equals Γ₁ Γ₂ ->
+  dom Γ₁ = dom Γ₂.
+Proof.
+  intros [s₁ f₁] [s₂ f₂].
+  simpls*.
+Qed.
+
+Hint Resolve 
+  eq_refl eq_sym eq_trans 
+  union_comm union_assoc
+  ok_empty ok_add ok_union ok_eq 
+  dom_add dom_union 
+: context_hints.
+Hint Rewrite union_empty_l union_empty_r : core.
+Hint Unfold ok equals empty union dom : context_hints.
+
+
+#[global] Instance Tightable_context : Tightable ctx := {| 
+  tight := fun (Γ : ctx) =>
+    let (_, f) := Γ in 
+    ∀ x, tight (f x)
+|}.
+
+Lemma union_tight_ctx :
+  ∀ Γ₁ Γ₂ Δ, 
+  tight Δ ->
+  equals (union Γ₁ Γ₂) Δ  ->
+  tight Γ₁ /\ tight Γ₂.
+Proof.
+  intros.
+  destruct Γ₁, Γ₂, Δ.
+  simpls; split_and_or_max;
+  intro x; specialize H with x; specialize H2 with x;
+  apply Types.mt_union_tight in H2 as [Htm Htm0]; autos*.
+Qed.
+
+Ltac tight_union_ctx Δ :=
+  match goal with 
+  | [H : equals (union ?Γ₁ ?Γ₂) Δ |- _] => 
+    let H_tight_Γ₁ := fresh "H_tight_Γ₁" in 
+    let H_tight_Γ₂ := fresh "H_tight_Γ₂" in 
+      apply union_tight_ctx in H as  [H_tight_Γ₁ H_tight_Γ₂]; eauto 
+  end.
+
+Lemma ok_get_equals :
+  ∀ Γ₁ Γ₂, 
+  ok Γ₁ -> ok Γ₂ -> 
+  equals Γ₁ Γ₂ <-> ∀ x, eq_multitype (get Γ₁ x) (get Γ₂ x).
+Proof.
+  split.
+  {
+    intros Heq x.
+    destruct Γ₁, Γ₂; simpls*.
+  }
+  {
+    asserts Heqnnil : (
+      ∀ mt1 mt2,
+        mt1 ≠ {{nil}} ->
+        eq_multitype mt1 mt2 ->
+        mt2 ≠ {{nil}}
+    ).
+    {
+      intros; destruct* mt1.
+      intro; substs. apply Types.eq_empty_is_empty in H2; autos*.
+    }
+    intros.
+    destruct Γ₁, Γ₂; split; simpls*.
+    apply fset_extens;
+    intros x Hin;
+    repeat match goal with 
+    | [H : ∀ _, _ |- _] => specialize H with x
+    end; split_and_or_max;
+    match goal with 
+    | [H : ?x \in ?v , H' : ?x \in ?v -> _ |- _] => apply H' in H
+    end;
+    match goal with 
+    | [H : ?mx ≠ {{nil}}, H' : eq_multitype ?mx ?mx2 |- _] => 
+        apply Heqnnil with (mt2 := mx2) in H
+    | [H : ?mx ≠ {{nil}}, H' : eq_multitype ?mx2 ?mx |- _] => 
+        use_equivalences; apply Heqnnil with (mt2 := mx2) in H
+    end; autos*.
+  }
+Qed.
+
