theories/Types/Types.v
@@ -1,24 +1,33 @@
-
 From Coq Require Import Unicode.Utf8_core.
 From Coq Require Import Lia.
-From Coq Require Import Lists.ListSet.
-From Coq Require Vector.
-Import Vector.VectorNotations.
-From Coq Require Import Classes.Equivalence.
-From Coq Require Import List.
-Import ListNotations.
-Require Import LogicSet.
-Require Import Tactics.
+From TLC Require Import LibLN LibTactics LibFset LibList LibRelation.
+From TTSB Require Import Tactics.
+From TTSB Require Import Classes.
+Create HintDb type_hints.
+
+
+Ltac auto_tilde :=
+  try (solve[ auto with type_hints
+            | intuition auto with type_hints ]).
+
+Ltac auto_star ::= 
+  try (solve [ eauto with type_hints 
+             | jauto 
+             | intuition eauto with type_hints ]).
 
 Parameter AtomicType : Set.
-Parameter X : set AtomicType.
+Parameter X : fset AtomicType.
 Parameter eqₐ : AtomicType -> AtomicType -> Prop.
 Parameter eqₐ_dec : 
   ∀ (t₁ t₂ : AtomicType),
   {eqₐ t₁ t₂} + {¬ eqₐ t₁ t₂}.
-Parameter eqₐ_Eq : 
-  Equivalence eqₐ.
+Parameter eqₐ_equiv : 
+  equiv eqₐ.
 Infix "≡ₐ" := eqₐ (at level 0).
+
+Hint Constructors equiv : type_hints.
+Hint Resolve eqₐ_equiv eqₐ_dec : type_hints.
+
 
 Inductive tight_constant := 
 | TC_Neutral : tight_constant
@@ -26,520 +35,90 @@ Inductive tight_constant :=
 .
 Inductive type :=
 | Ty_Tight (t : tight_constant) : type
-| Ty_Atomic (t : AtomicType) : (set_In t X) -> type
+| Ty_Atomic (t : AtomicType) : (t \in X) -> type
 | Ty_Fun : multitype -> type -> type 
-| Ty_Mult : multitype -> type
 with multitype :=
 | MT_Empty : multitype
 | MT_Cons (t : type) (mt : multitype) : multitype
 .
-
 Scheme type_mut_ind := Induction for type Sort Type
 with multitype_mut_ind := Induction for multitype Sort Type.
 
+Hint Constructors tight_constant type multitype : type_hints.
 
-
-
-
-
-
-
-Fixpoint MT_Union (mt₁ mt₂ : multitype) : multitype :=
+Fixpoint union (mt₁ mt₂ : multitype) : multitype :=
   match mt₁ with 
-  | MT_Empty => mt₂ 
-  | MT_Cons t mt₁ => MT_Cons t (MT_Union mt₁ mt₂)
-  end 
-.
+  | MT_Empty => mt₂
+  | MT_Cons t mt₁' => MT_Cons t (union mt₁' mt₂) 
+  end.
 
-Fixpoint is_tight_type (t : type) : Prop :=
-  match t with
-  | Ty_Tight _ => True 
-  | Ty_Atomic _ _ => False
-  | Ty_Fun _ _ => False
-  | Ty_Mult mt => is_tight_multitype mt
-  end
-with is_tight_multitype (mt : multitype) : Prop :=
+Hint Unfold union : type_hints.
+
+#[global] Instance Tight_type : Tightable type := {
+  tight := 
+    fun t => 
+    match t with
+    | Ty_Tight _ => True 
+    | Ty_Atomic _ _ => False
+    | Ty_Fun _ _ => False
+    end
+}.
+
+Fixpoint tight_aux (mt : multitype) : Prop := 
   match mt with 
   | MT_Empty => True
-  | MT_Cons t mt' => (is_tight_type t) /\ (is_tight_multitype mt')
+  | MT_Cons t mt' => (tight t) /\ (tight_aux mt')
   end.
-
-Create HintDb permutation_hints.
-
-  Inductive permutationₜ : type -> type -> Prop :=
-  | P_Tight : 
-      ∀ (t : tight_constant), 
-      permutationₜ (Ty_Tight t) (Ty_Tight t)
-  | P_Atomic :
-      ∀ (t₁ t₂ : AtomicType) 
-        (prf₁ : set_In t₁ X) (prf₂ : set_In t₂ X),
-      eqₐ t₁ t₂ -> 
-      permutationₜ (Ty_Atomic t₁ prf₁) (Ty_Atomic t₂ prf₂)
-  | P_Fun : 
-      ∀ (mt₁ mt₂ : multitype) (t₁ t₂ : type),
-      permutationₘ mt₁ mt₂ -> 
-      permutationₜ t₁ t₂ -> 
-      permutationₜ (Ty_Fun mt₁ t₁) (Ty_Fun mt₂ t₂)
-  | P_Mult : 
-      ∀ (mt₁ mt₂ : multitype), 
-      permutationₘ mt₁ mt₂ -> 
-      permutationₜ (Ty_Mult mt₁) (Ty_Mult mt₂)
-  with permutationₘ : multitype -> multitype -> Prop :=
-  | P_MT_Empty : permutationₘ (MT_Empty) (MT_Empty)
-  | P_MT_Cons : 
-      ∀ (mt₁ mt₂ : multitype) (t₁ t₂ : type),
-      permutationₜ t₁ t₂ -> 
-      permutationₘ mt₁ mt₂ -> 
-      permutationₘ (MT_Cons t₁ mt₁) (MT_Cons t₂ mt₂)
-  | P_MT_Swap : 
-      ∀ (t₁ t₂ : type) (mt : multitype),
-        permutationₘ 
-          (MT_Cons t₁ (MT_Cons t₂ mt))
-          (MT_Cons t₂ (MT_Cons t₁ mt))
-  | P_MT_Trans :
-      ∀ (mt₁ mt₂ mt₃ : multitype),
-      permutationₘ mt₁ mt₂ ->
-      permutationₘ mt₂ mt₃ ->
-      permutationₘ mt₁ mt₃
-  .
-  Hint Constructors permutationₜ : permutation_hints.
-  Hint Constructors permutationₘ : permutation_hints.
-  Scheme permutationₜ_mut_ind := Induction for permutationₜ Sort Prop
-  with permutationₘ_mut_ind := Induction for permutationₘ Sort Prop.
-
-  Check permutationₜ_mut_ind.
-  Theorem permₜ_refl : ∀ (t : type), permutationₜ t t.
-  Proof with eauto with permutation_hints.
-    destruct eqₐ_Eq.
-    unshelve induction t 
-      using type_mut_ind 
-      with (P0 := fun mt => permutationₘ mt mt)...
-  Qed.
-
-  Theorem permₘ_refl : ∀ (mt : multitype), permutationₘ mt mt.
-  Proof with eauto with permutation_hints.
-    destruct eqₐ_Eq.
-    einduction mt 
-      using multitype_mut_ind with (P := fun t => permutationₜ t t)...
-  Qed.
-
-  Theorem permₜ_sym : 
-    ∀ (t₁ t₂ : type), 
-    permutationₜ t₁ t₂ ->
-    permutationₜ t₂ t₁.
-  Proof with eauto with permutation_hints.
-    intros * H_perm.
-    destruct eqₐ_Eq.
-    pose (
-      P0 (mt₁ mt₂ : multitype ) (H_perm : permutationₘ mt₁ mt₂) := 
-      permutationₘ mt₂ mt₁ 
-    ).
-    induction H_perm 
-      using permutationₜ_mut_ind 
-      with (P0 := P0); unfold P0...
-  Qed.
-  Theorem permₘ_sym : 
-    ∀ (mt₁ mt₂ : multitype), 
-    permutationₘ mt₁ mt₂ ->
-    permutationₘ mt₂ mt₁.
-  Proof with eauto with permutation_hints.
-    intros * H_perm.
-    destruct eqₐ_Eq.
-    pose (
-      P (t₁ t₂ : type ) (H_perm : permutationₜ t₁ t₂) := permutationₜ t₂ t₁ 
-    ).
-    induction H_perm 
-      using permutationₘ_mut_ind 
-      with (P := P); unfold P...
-  Qed.
-
-  Theorem permₜ_trans : 
-    ∀ (t₁ t₂ t₃ : type), 
-    permutationₜ t₁ t₂ -> 
-    permutationₜ t₂ t₃ -> 
-    permutationₜ t₁ t₃.
-  Proof with eauto with permutation_hints.
-    destruct eqₐ_Eq.
-    intros * H_perm1.
-    generalize dependent t₃.
-    pose (
-      P0 (mt₁ mt₂ : multitype) (H_perm : permutationₘ mt₁ mt₂) :=
-        ∀ (mt₃ : multitype), permutationₘ mt₂ mt₃ -> permutationₘ mt₁ mt₃
-    ).
-    induction H_perm1 
-      using permutationₜ_mut_ind 
-      with (P0 := P0); unfold P0; try (
-        intros t₃ H_perm2;
-        inversion H_perm2;
-        eauto with permutation_hints;
-        fail
-      )...
-  Qed.
-
-  Theorem permₘ_trans : 
-    ∀ (mt₁ mt₂ mt₃ : multitype), 
-    permutationₘ mt₁ mt₂ -> 
-    permutationₘ mt₂ mt₃ -> 
-    permutationₘ mt₁ mt₃.
-  Proof with eauto with permutation_hints.
-    destruct eqₐ_Eq.
-    intros * H_perm1.
-    generalize dependent mt₃.
-    pose (
-      P (t₁ t₂ : type) (H_perm : permutationₜ t₁ t₂) :=
-        ∀ (t₃ : type), permutationₜ t₂ t₃ -> permutationₜ t₁ t₃
-    ).
-    induction H_perm1 
-      using permutationₘ_mut_ind
-      with (P := P); unfold P; try (
-        intros t₃ H_perm2; 
-        inversion H_perm2; eauto with permutation_hints; fail
-      )...
-  Qed.
-
-  Hint Resolve permₜ_refl permₜ_sym permₜ_trans: permutation_hints.
-  Hint Resolve permₘ_refl permₘ_sym permₘ_trans: permutation_hints.
-
-Module Type MULTITYPE.
-  Parameter T : Set.
-  Parameter eq : T -> T -> Prop. 
-  Parameter union : T -> T -> T.
-
-  Axiom eq_refl : ∀ (t : T), eq t t.
-  Axiom eq_sym : ∀ (t₁ t₂ : T), eq t₁ t₂ -> eq t₂ t₁.
-  Axiom eq_trans : ∀ (t₁ t₂ t₃ : T), eq t₁ t₂ -> eq t₂ t₃ -> eq t₁ t₃.
-  Axiom union_comm : ∀ mt₁ mt₂, eq (union mt₁ mt₂) (union mt₂ mt₁).
-  Axiom union_assoc : 
-    ∀ mt₁ mt₂ mt₃, 
-    eq 
-      (union (union mt₁ mt₂) mt₃) 
-      (union mt₁ (union mt₂ mt₃)). 
-  
-  Axiom eq_union : 
-    ∀ t₁ t₁' t₂ t₂', 
-    eq t₁ t₁' -> 
-    eq t₂ t₂' -> 
-    eq (union t₁ t₂) (union t₁' t₂').
-  
+#[global] Instance Tight_multitype : Tightable multitype := {
+  tight := tight_aux
+}.
 
 
-End MULTITYPE.
-
-
-Module Multitype <: MULTITYPE.
-  Definition T := multitype.
-  Definition eq := permutationₘ.
-  Definition union := MT_Union.
-
-   
-  Theorem eq_refl : ∀ (t : T), eq t t. 
-  Proof. 
-    unfold eq.
-    eauto with permutation_hints.
-  Qed.
-
-  Theorem eq_sym : ∀ (t₁ t₂ : T), eq t₁ t₂ -> eq t₂ t₁.
-  Proof. 
-    unfold eq.
-    eauto with permutation_hints.
-  Qed.
-
-  Theorem eq_trans : ∀ (t₁ t₂ t₃ : T), eq t₁ t₂ -> eq t₂ t₃ -> eq t₁ t₃.
-  Proof. 
-    unfold eq.
-    eauto with permutation_hints.
-  Qed.
-
-  
-  Lemma union_empty_r : 
-    ∀ (mt : multitype),
-      (union mt MT_Empty) = mt.
-  Proof with eauto with permutation_hints.
-    unfold eq.
-    induction mt; simpl...
-    rewrite IHmt...
-  Qed.
-
-  Lemma union_perm_tail : 
-    ∀ (mt₁ mt₂ mt₂': multitype), 
-    eq mt₂ mt₂' -> 
-    eq (union mt₁ mt₂) (union mt₁ mt₂').
-  Proof with eauto with permutation_hints.
-    unfold eq.
-    induction mt₁...
-  Qed.
-
-  Lemma union_perm_head : 
-    ∀ (mt₁ mt₁' mt₂ : multitype),
-    eq mt₁ mt₁' -> 
-    eq (union mt₁ mt₂) (union mt₁' mt₂).
-  Proof with eauto with permutation_hints.
-    unfold eq.
-    intros * H_perm.
-    induction H_perm...
-  Qed.
-
-
-  Lemma union_perm_app : 
-    ∀ (mt₁ mt₁' mt₂ mt₂' : multitype),
-    eq mt₁ mt₁' ->
-    eq mt₂ mt₂' ->
-    eq (union mt₁ mt₂) (union mt₁' mt₂').
-  Proof with unfold eq; eauto with permutation_hints.
-    intros.
-    eapply permₘ_trans.
-    - apply union_perm_head...
-    - apply union_perm_tail...
-  Qed. 
-
-  Lemma union_insert : 
-    ∀ (mt₁ mt₁' mt₂ mt₂' : multitype) (t t' : type),
-    eq mt₁ mt₁' -> 
-    eq mt₂ mt₂' -> 
-    permutationₜ t t' -> 
-    eq 
-      (union mt₁ (MT_Cons t mt₂))
-      (union mt₁' (MT_Cons t' mt₂'))
-    .
-  Proof with unfold eq; eauto 3 with permutation_hints.
-    unfold eq.
-    intros * H_eq_1 H_eq_2 H_perm.
-    induction H_eq_1; apply union_perm_app...
-  Qed.
-
-  Lemma union_cons : 
-    ∀ (mt : multitype) (t : type),
-    eq (MT_Cons t mt) (union mt (MT_Cons t MT_Empty)).
-  Proof with unfold eq; eauto with permutation_hints.
-    intros.
-    induction mt...
-  Qed.
-
-
-  Theorem union_assoc : 
+Inductive eq_type : type -> type -> Prop :=
+| Eq_Tight : 
+    ∀ (t : tight_constant), 
+    eq_type (Ty_Tight t) (Ty_Tight t)
+| Eq_Atomic :
+    ∀ (t₁ t₂ : AtomicType) 
+      (prf₁ : t₁ \in X) (prf₂ : t₂ \in X),
+    eqₐ t₁ t₂ -> 
+    eq_type (Ty_Atomic t₁ prf₁) (Ty_Atomic t₂ prf₂)
+| Eq_Fun : 
+    ∀ (mt₁ mt₂ : multitype) (t₁ t₂ : type),
+    eq_multitype mt₁ mt₂ -> 
+    eq_type t₁ t₂ -> 
+    eq_type (Ty_Fun mt₁ t₁) (Ty_Fun mt₂ t₂)
+with eq_multitype : multitype -> multitype -> Prop :=
+| Eq_MT_Empty : eq_multitype (MT_Empty) (MT_Empty)
+| Eq_MT_Cons : 
+    ∀ (mt₁ mt₂ : multitype) (t₁ t₂ : type),
+    eq_type t₁ t₂ -> 
+    eq_multitype mt₁ mt₂ -> 
+    eq_multitype (MT_Cons t₁ mt₁) (MT_Cons t₂ mt₂)
+| Eq_MT_Swap : 
+    ∀ (t₁ t₂ : type) (mt : multitype),
+      eq_multitype 
+        (MT_Cons t₁ (MT_Cons t₂ mt))
+        (MT_Cons t₂ (MT_Cons t₁ mt))
+| Eq_MT_Trans :
     ∀ (mt₁ mt₂ mt₃ : multitype),
-    eq 
-      (union (union mt₁ mt₂) mt₃)
-      (union mt₁ (union mt₂ mt₃)).
-  Proof with eauto with permutation_hints.
-    unfold eq.
-    intros.
-    induction mt₁...
-  Qed.
+    eq_multitype mt₁ mt₂ ->
+    eq_multitype mt₂ mt₃ ->
+    eq_multitype mt₁ mt₃
+.
+Check eq_multitype_ind.
+Hint Constructors eq_type eq_multitype : type_hints.
+Scheme eq_type_mut_ind := Induction for eq_type Sort Prop
+with eq_multitype_mut_ind := Induction for eq_multitype Sort Prop.
 
+Ltac eq_type_induction eq P0 := 
+  induction eq using eq_type_mut_ind with (P0:=P0); unfold P0 in *; clear P0.
 
-  Theorem union_comm : ∀ mt₁ mt₂, eq (union mt₁ mt₂) (union mt₂ mt₁).
-  Proof with 
-    eauto
-    using 
-      eq_sym, eq_trans, eq_refl,
-      union_empty_r, union_assoc, union_cons,
-      union_perm_head
-    with permutation_hints.
-    unfold eq.
-    induction mt₁ as [|h₁ mt₁']; simpl; intro mt₂...
-    - apply eq_sym. rewrite union_empty_r...
-    - eapply eq_trans with (MT_Cons h₁ (union mt₂ mt₁'))...
-      + apply P_MT_Cons...
-      + apply eq_trans with (union (union mt₂ (MT_Cons h₁ MT_Empty)) mt₁')...
-  Qed.
+Ltac eq_multitype_induction eq P := 
+  induction eq using eq_multitype_mut_ind with (P:=P); unfold P in *; clear P.
 
-  Lemma eq_union_left : 
-    ∀ t₁ t₁' t₂, 
-    eq t₁ t₁'-> 
-    eq (union t₁ t₂) (union t₁' t₂).
-  Proof with eauto with permutation_hints.
-    Hint Unfold eq : core.
-    intros.
-    induction H...
-  Qed.
-
-  Lemma eq_union_right : 
-    ∀ t₁ t₂ t₂', 
-    eq t₂ t₂'-> 
-    eq (union t₁ t₂) (union t₁ t₂').
-  Proof with eauto using eq_union_left, union_comm with permutation_hints.
-    unfold eq.
-    intros * H_eq.
-    apply eq_trans with (union t₂ t₁)...
-    apply eq_trans with (union t₂' t₁)...
-  Qed.
-
-  Lemma eq_union : 
-    ∀ t₁ t₁' t₂ t₂', 
-    eq t₁ t₁' -> 
-    eq t₂ t₂' -> 
-    eq (union t₁ t₂) (union t₁' t₂').
-  Proof with eauto using eq_union_left, eq_union_right with permutation_hints.
-    Hint Unfold eq : core.
-    intros * H_eq_1 H_eq_2.
-    apply eq_trans with (union t₁ t₂')...
-  Qed.
-
-  Fixpoint size (mt : multitype) :=
-  match mt with 
-  | MT_Empty => 0 
-  | MT_Cons _ mt' => 1 + size mt'
-  end.
-  
-End Multitype.
-
-
-
-
-Module Context (MT : MULTITYPE).
-  Definition t := list MT.T.
-
-  Inductive union : t -> t -> t -> Type :=
-  | Union_Nil : union [] [] [] 
-  | Union_Cons : 
-    ∀  Γ₁ Γ₂ Γᵣ mt₁ mt₂ mtu, 
-    union Γ₁ Γ₂ Γᵣ -> 
-    MT.eq (MT.union  mt₁ mt₂) mtu ->
-    union (mt₁ :: Γ₁) (mt₂ :: Γ₂) (mtu :: Γᵣ)
-  .
-  Hint Constructors union : core.
-
-  Fixpoint eq (Γ₁ Γ₂ : t) : Prop :=
-    match Γ₁, Γ₂ with 
-    | [], [] => True
-    | [], _::_ | _::_, [] => False
-    | h₁::t₁, h₂::t₂ => (MT.eq h₁ h₂) /\ (eq t₁ t₂)
-    end.
-  Hint Unfold eq : core.
-
-
-  Lemma eq_empty_l : ∀ Γ, eq [] Γ -> Γ = [].
-  Proof with eauto.
-    induction Γ; intros...
-    inversion H.
-  Qed.
-
-  Lemma eq_empty_r : ∀ Γ, eq Γ [] -> Γ = [].
-  Proof with eauto.
-    induction Γ; intros...
-    inversion H.
-  Qed.
-
-  Lemma eq_refl : ∀ Γ, eq Γ Γ.
-  Proof with eauto.
-    induction Γ; simpl...
-    split...
-    apply MT.eq_refl.
-  Qed.
-  
-
-  Lemma eq_sym : 
-    ∀ (Γ₁ Γ₂ : t),
-    eq Γ₁ Γ₂ ->
-    eq Γ₂ Γ₁.
-  Proof with eauto.
-    induction Γ₁ as [| mt₁ Γ₁]; intros [| mt₂ Γ₂ ] H_eq; simpl in *; repeat split_and...
-    apply MT.eq_sym...
-  Qed.
-
-
-  Lemma eq_trans : 
-    ∀ (Γ₁ Γ₂ Γ₃: t),
-    eq Γ₁ Γ₂ ->
-    eq Γ₂ Γ₃ ->
-    eq Γ₁ Γ₃.
-  Proof with eauto.
-    induction Γ₁ as [| mt₁ Γ₁]; intros [| mt₂ Γ₂ ] [| mt₃ Γ₃ ] H_eq1 H_eq2; simpl in *; repeat split_and; try contradiction...
-    eapply MT.eq_trans...
-  Qed.
-
-  Theorem union_comm : 
-    ∀ (Γ₁ Γ₂ Γᵣ₁ Γᵣ₂: t),
-    union Γ₁ Γ₂ Γᵣ₁ -> 
-    union Γ₂ Γ₁ Γᵣ₂ -> 
-    eq Γᵣ₁ Γᵣ₂.
-  Proof with eauto.
-    intros * H_union_1. generalize dependent Γᵣ₂.
-    induction H_union_1; intros * H_union_2; inversion H_union_2; subst; simpl...
-    split...
-    eapply MT.eq_trans...
-    apply MT.eq_sym.
-    apply MT.eq_trans with (MT.union mt₁ mt₂)...
-    apply MT.union_comm.
-  Qed.
-
-  Ltac inversion_eq_list := 
-    match goal with 
-    | [H : _ :: _ = _ :: _ |- _] => inversion H; clear H; subst
-    end.
-
-  Theorem union_assoc : 
-    ∀ (Γ₁ Γ₂ Γ₃ Γ₁₂ Γ₁₂_₃ Γ₂₃ Γ₁_₂₃ : t),
-    union Γ₁ Γ₂ Γ₁₂ -> 
-    union Γ₁₂ Γ₃ Γ₁₂_₃ -> 
-    union Γ₂ Γ₃ Γ₂₃ -> 
-    union Γ₁ Γ₂₃ Γ₁_₂₃ -> 
-    eq Γ₁₂_₃ Γ₁_₂₃.
-  Proof with eauto using MT.eq_refl, MT.eq_sym, MT.eq_trans, MT.union_assoc, MT.eq_union.
-  Hint Unfold eq : core.
-  intros * H_union_1_2.
-  generalize dependent Γ₃.
-  generalize dependent Γ₁₂_₃. 
-  generalize dependent Γ₂₃.
-  generalize dependent Γ₁_₂₃.
-  induction H_union_1_2; intros * H_union_12_3 H_union_2_3 H_union_1_23; inversion H_union_12_3; inversion H_union_2_3; inversion H_union_1_23; subst...
-  simpl.
-  repeat inversion_eq_list.
-  (* inversion H8; inversion H14; subst. *)
-  split...
-  apply MT.eq_trans with (MT.union mt₁ mtu1)...
-  apply MT.eq_trans with (MT.union mtu mt₂0)...
-  apply MT.eq_trans with (MT.union mt₁ (MT.union mt₂ mt₂0))...
-Qed.
-
-
-
-  Lemma eq_union_left : 
-    ∀ Γ₁ Γ₁' Γ₂ Γᵣ, 
-    eq Γ₁ Γ₁'-> 
-    union Γ₁ Γ₂ Γᵣ -> 
-    union Γ₁' Γ₂ Γᵣ
-    .
-  Proof with eauto 6 using MT.eq_union, MT.eq_sym, MT.eq_refl, MT.eq_trans, Union_Cons with permutation_hints.
-    induction Γ₁ as [ | mt₁ Γ₁ IHΓ]; intros [| mt₁' Γ₁'] [ | mt₂ Γ₂] [| mtᵣ Γᵣ] H_eq H_u; inversion H_u; try inversion H_eq; subst; simpl...
-  Qed.
-
-  Lemma eq_union_right : 
-    ∀ Γ₁ Γ₂ Γ₂' Γᵣ, 
-    eq Γ₂ Γ₂'-> 
-    union Γ₁ Γ₂ Γᵣ -> 
-    union Γ₁ Γ₂' Γᵣ
-    .
-  Proof with eauto 6 using MT.eq_union, MT.eq_sym, MT.eq_refl, MT.eq_trans, Union_Cons with permutation_hints.
-    induction Γ₁ as [ | mt₁ Γ₁ IHΓ]; intros [| mt₂ Γ₂] [ | mt₂' Γ₂'] [| mtᵣ Γᵣ] H_eq H_u; inversion H_u; try inversion H_eq; subst; simpl...
-  Qed.
-
-  Lemma eq_union : 
-    ∀ Γ₁ Γ₁' Γ₂ Γ₂' Γᵣ, 
-    eq Γ₁ Γ₁'-> 
-    eq Γ₂ Γ₂'-> 
-    union Γ₁ Γ₂ Γᵣ -> 
-    union Γ₁' Γ₂' Γᵣ.
-  Proof.
-    eauto using eq_trans, eq_union_left, eq_union_right with permutation_hints.
-  Qed.    
-
-End Context.
-
-Module Ctx := Context Multitype.
-
-
-Fixpoint is_tight_context(Γ : Ctx.t) : Prop :=
-  match Γ with 
-  | [] => True 
-  | h::t => (is_tight_multitype h) /\ (is_tight_context t) 
-  end.
-
-
-Hint Unfold is_tight_type is_tight_multitype is_tight_context  : core.
-Notation "a ⊎ b" := (Multitype.union a b) (at level 0).
-Notation "a '⊎c' b ≡ c" := (Ctx.union a b c) (at level 0).
+Module TypesNotations.
+Notation "a ⊎ b" := (union a b) (at level 0).
 
 Declare Custom Entry multitype. 
 
@@ -553,99 +132,327 @@ Notation " t ; mt" := (MT_Cons t mt) (in custom multitype at level 90, mt custom
 Notation "mt |-> t" := (Ty_Fun mt t) (at level 99, right associativity).
 Notation "{{ mt }} |-> t" := (Ty_Fun mt t) (in custom multitype at level 80, right associativity).
 
+End TypesNotations.
 
+Import TypesNotations.
 
-Fixpoint In (t : type) (mt : multitype) : Prop :=
-  match mt with 
-  | {{ nil }} => False
-  | {{ h ; mt }} => (permutationₜ t h) \/ (In t mt)
-  end.
+Check eq_type_mut_ind.
 
-Lemma mt_eq_in : 
-  ∀ (t : type) (mt₁ mt₂ : multitype),
-  Multitype.eq mt₁ mt₂ -> 
-  In t mt₁ ->
-  In t mt₂.
-Proof with eauto with permutation_hints.
-  intros * H_eq H_in.
-  induction H_eq...
-  - inversion H_in.
-    + left...
-    + right...
-  - inversion H_in.
-    + right. left...
-    + inversion H.
-      * left...
-      * right; right...
+#[global] Instance Equiv_eq_type : Equivalence eq_type.
+Proof.
+  constructor.
+  - intro t; destruct eqₐ_equiv;
+    pose (P0 mt := eq_multitype mt mt).
+    induction t
+      using type_mut_ind 
+      with (P0 := P0); unfolds P0; clear P0; autos*.
+  - intros t₁ t₂ Heq; destruct eqₐ_equiv.
+    pose (
+      P0 (mt₁ mt₂ : multitype ) (Heq : eq_multitype mt₁ mt₂) := 
+      eq_multitype mt₂ mt₁ 
+    );
+    eq_type_induction Heq P0; autos*.
+  - intros t₁ t₂ t₃ Heq; destruct eqₐ_equiv;
+    pose (
+    P0 (mt₁ mt₂ : multitype) (Heq : eq_multitype mt₁ mt₂) :=
+      ∀ (mt₃ : multitype), eq_multitype mt₂ mt₃ -> eq_multitype mt₁ mt₃
+  ).
+  gen t₃.
+  eq_type_induction Heq P0; 
+  intros t₃ Heq2; inverts* Heq2.
 Qed.
 
 
-Ltac permutationₜ_induction perm P0 := 
-  induction perm using permutationₜ_mut_ind with (P0:=P0); unfold P0 in *; clear P0.
+#[global] Instance Equiv_eq_multitype : Equivalence eq_multitype. 
+Proof.
+  destruct Equiv_eq_type.
+  constructor.
+  - substs.
+    intro t. 
+    induction t; autos*.
+  - intros t₁ t₂ Heq; inductions Heq; autos*.
+  - intros t₁ t₂ t₃ Heq; gen t₃; inductions Heq; autos*.
+Qed.
 
-Ltac permutationₘ_induction perm P := 
-  induction perm using permutationₘ_mut_ind with (P:=P); unfold P in *; clear P.
+Ltac use_equivalences_type := 
+  destruct Equiv_eq_type 
+    as [eq_type_refl eq_type_sym eq_type_trans];
+  destruct Equiv_eq_multitype 
+    as [eq_multitype_refl eq_multitype_sym eq_multitype_trans].
+
+Ltac use_equivalences ::= use_equivalences_type.
+
+Generalizable Variables A rel.
+
+Lemma eq_empty_is_empty :
+  ∀ mt, eq_multitype mt MT_Empty -> mt = MT_Empty.
+Proof.
+  introv Heq.
+  inductions Heq; autos.
+Qed.
+
+Lemma union_empty_r : 
+  ∀ (mt : multitype),
+    (union mt MT_Empty) = mt.
+Proof.
+  induction mt; simpls*.
+  rewrites* IHmt.
+Qed.
+
+
+Lemma nnil_union : 
+  ∀ mt1 mt2, 
+  mt1 ≠ {{ nil }} \/ mt2 ≠ {{ nil }} <->
+  mt1 ⊎ mt2 ≠ {{nil}}.
+Proof.
+  split.
+  - introv [Hmt1_nnil | Hmt2_nnil]; inductions mt1; autos*;
+    absurd.
+  - introv H_nnil;
+    destruct mt1; simpls*.
+    left; absurd.
+Qed.
+
+Lemma nil_eq_union :
+  ∀ mt1 mt2, 
+  mt1 = {{ nil }} /\ mt2 = {{ nil }} <->
+  mt1 ⊎ mt2 = {{nil}}.
+Proof.
+  split.
+  - introv [Hmt1_nil Hmt2_nil]; inductions mt1; 
+    repeat match goal with 
+    | [H : _ = {{nil}} |- _] => rewrite H 
+    | [H : {{nil}} = _ |- _] => rewrite <- H
+    end; simpls*.
+  - introv H_nil;
+    destruct mt1; simpls*.
+    inversion H_nil.
+Qed.
+
+Lemma union_perm_tail : 
+  ∀ (mt₁ mt₂ mt₂': multitype), 
+  eq_multitype mt₂ mt₂' -> 
+  eq_multitype (union mt₁ mt₂) (union mt₁ mt₂').
+Proof.
+  use_equivalences.
+  introv Heq.
+  inductions mt₁; autos*.
+Qed.
+
+
+Lemma union_perm_head : 
+  ∀ (mt₁ mt₁' mt₂ : multitype),
+  eq_multitype mt₁ mt₁' -> 
+  eq_multitype (union mt₁ mt₂) (union mt₁' mt₂).
+Proof with eauto with permutation_hints.
+  use_equivalences.
+  introv Heq.
+  inductions Heq; simpls*.
+Qed.
+
+Lemma union_perm : 
+  ∀ (mt₁ mt₁' mt₂ mt₂' : multitype),
+  eq_multitype mt₁ mt₁' ->
+  eq_multitype mt₂ mt₂' ->
+  eq_multitype (union mt₁ mt₂) (union mt₁' mt₂').
+Proof.
+  use_equivalences.
+  intros.
+  unfolds trans.
+  eapply eq_multitype_trans.
+  - applys* union_perm_head.
+  - applys* union_perm_tail.
+Qed.
+
+
+
+Lemma union_insert : 
+  ∀ (mt₁ mt₁' mt₂ mt₂' : multitype) (t t' : type),
+  eq_multitype mt₁ mt₁' -> 
+  eq_multitype mt₂ mt₂' -> 
+  eq_type t t' -> 
+  eq_multitype
+    (union mt₁ (MT_Cons t mt₂))
+    (union mt₁' (MT_Cons t' mt₂'))
+  .
+Proof.
+  use_equivalences.
+  introv Heq1 Heq2 Heqt.
+  induction Heq1; applys* union_perm.
+Qed.
+
+Lemma union_cons : 
+  ∀ (mt : multitype) (t : type),
+  eq_multitype (MT_Cons t mt) (union mt (MT_Cons t MT_Empty)).
+Proof.
+  use_equivalences.
+  intros.
+  inductions mt; simpls*.
+Qed.
+
+
+Theorem union_assoc : 
+  ∀ (mt₁ mt₂ mt₃ : multitype),
+  eq_multitype 
+    (union (union mt₁ mt₂) mt₃)
+    (union mt₁ (union mt₂ mt₃)).
+Proof.
+  use_equivalences.
+  intros.
+  inductions mt₁; autos*.
+Qed.
+
+Theorem union_comm : 
+  ∀ mt₁ mt₂, eq_multitype (union mt₁ mt₂) (union mt₂ mt₁).
+  Proof.
+    use_equivalences.
+    hint union_empty_r, union_assoc, union_cons, union_perm_head.
+    induction mt₁ as [|h₁ mt₁']; intro mt₂.
+    - rewrites* union_empty_r.
+    - autos*.
+  Qed.
+
+
+Lemma eq_union_left : 
+  ∀ mt₁ mt₁' mt₂, 
+  eq_multitype mt₁ mt₁'-> 
+  eq_multitype (union mt₁ mt₂) (union mt₁' mt₂).
+Proof with eauto with permutation_hints.
+  use_equivalences.
+  introv Heq.
+  inductions Heq; autos*.
+Qed.
+
+
+
+Lemma eq_union_right: 
+  ∀ mt₁ mt₂ mt₂', 
+  eq_multitype mt₂ mt₂'-> 
+  eq_multitype (union mt₁ mt₂) (union mt₁ mt₂').
+Proof.
+  introv Heq.
+  hint eq_union_left, union_comm.
+  apply transitive with (a₂ := union mt₂ mt₁); autos*.
+Qed.
+
+Lemma eq_union : 
+  ∀ t₁ t₁' t₂ t₂', 
+  eq_multitype t₁ t₁' -> 
+  eq_multitype t₂ t₂' -> 
+  eq_multitype (union t₁ t₂) (union t₁' t₂').
+Proof.
+  introv Heq1 Heq2.
+  hint eq_union_left, eq_union_right, union_comm.
+  autos*.
+Qed.
+
+Fixpoint size_aux (mt : multitype) : nat := match mt with 
+    | MT_Empty => 0 
+    | MT_Cons _ mt' => 1 + size_aux mt'
+end.
+
+#[global] Instance Sized_multitype : Sized multitype := { 
+  size := size_aux
+}.
+
+Lemma eq_size : 
+  ∀ M₁ M₂,
+  eq_multitype M₁ M₂ -> 
+  size M₁ = size M₂.
+Proof.
+  intros.
+  induction* H; simpls.
+  - fequals. 
+  - etransitivity; eassumption.
+Qed.
+
+Lemma size_union :
+  ∀ M₁ M₂,
+  size (M₁ ⊎ M₂) = size M₁ + size M₂.
+Proof.
+  induction M₁; simpls; introv; try rewrite IHM₁; reflexivity.
+Qed. 
+
+Fixpoint In (t : type) (mt : multitype) : Prop := 
+  match mt with 
+  | {{ nil }} => False
+  | {{ h ; mt }} => (eq_type t h) \/ (In t mt)
+  end.
+
+Lemma eq_in :
+  ∀ (t : type) (mt₁ mt₂ : multitype),
+  eq_multitype mt₁ mt₂ -> 
+  In t mt₁ ->
+  In t mt₂.
+Proof.
+  use_equivalences.
+  intros * Heq Hin.
+  induction Heq; autos*;
+  inverts Hin; simpls*.
+Qed.
+
+
 
 Lemma eq_tight : 
   ∀ t₁ t₂, 
-  permutationₜ t₁ t₂ ->
-  is_tight_type t₁ -> 
-  is_tight_type t₂.
-Proof with eauto using mt_eq_in with permutation_hints.
-  intros * H_perm.
-  pose (P0 (mt₁ mt₂ : multitype) (H_permₘ : permutationₘ mt₁ mt₂) := is_tight_multitype mt₁ -> is_tight_multitype mt₂).
-  permutationₜ_induction H_perm P0; try (intro H_tight; split; inversion H_tight as [H_tight_t H_tight_mt]; try inversion H_tight_mt; eauto using mt_eq_in with permutation_hints; fail)...
+  eq_type t₁ t₂ ->
+  tight t₁ -> 
+  tight t₂.
+Proof with eauto using eq_in with permutation_hints.
+  intros * Heq.
+  pose (P0 (mt₁ mt₂ : multitype) (Heqₘ : eq_multitype mt₁ mt₂) := tight mt₁ -> tight mt₂).
+  eq_type_induction Heq P0; intros;
+  repeat match goal with 
+  | [H : tight {{ _ ; _}} |- _] => destruct H
+  | [ _: _ |- tight {{ _ ; _}}] => split
+  end; simpls; split_and_or_max; autos*.
 Qed.
 
 Lemma eq_tight_multitype : 
   ∀ mt₁ mt₂, 
-  permutationₘ mt₁ mt₂ ->
-  is_tight_multitype mt₁ -> 
-  is_tight_multitype mt₂.
-Proof with eauto using mt_eq_in with permutation_hints.
-  intros * H_perm.
-  pose (P (t₁ t₂ : type) (H_permₜ : permutationₜ t₁ t₂) := is_tight_type t₁ -> is_tight_type t₂).
-  permutationₘ_induction H_perm P; try (intro H_tight; split; inversion H_tight as [H_tight_t H_tight_mt]; try inversion H_tight_mt; repeat apply and_set_intro; eauto using mt_eq_in with permutation_hints; fail)...
-Qed.
-
-
-Lemma Ctx_eq_tight :
-  ∀ (Γ₁ Γ₂ : Ctx.t), Ctx.eq Γ₁ Γ₂ -> is_tight_context Γ₁ -> is_tight_context Γ₂.
-Proof with eauto using mt_eq_in, eq_tight, eq_tight_multitype with permutation_hints.
-  induction Γ₁; intros; destruct Γ₂; simpl in *; destruct H, H0...
+  eq_multitype mt₁ mt₂ ->
+  tight mt₁ -> 
+  tight mt₂.
+Proof.
+  intros * Heq.
+  pose (P (t₁ t₂ : type) (Heqₜ : eq_type t₁ t₂) := tight t₁ -> tight t₂).
+  eq_multitype_induction Heq P; autos*; intros Htight;
+  simpls; split_and_or; autos*.
 Qed.
 
 
 Lemma mt_union_tight :
   ∀ (mt₁ mt₂ mt : multitype), 
-    Multitype.eq (mt₁ ⊎ mt₂) mt -> 
-    is_tight_multitype mt -> 
-    is_tight_multitype mt₁ /\ is_tight_multitype mt₂.
-Proof with eauto using mt_eq_in, eq_tight, eq_tight_multitype with permutation_hints.
-  induction mt₁; intros; simpl.
-  - split...
-  - change {{` t `; ` mt₁ `}} with (Multitype.union {{t ; nil}} mt₁) in *.
-    assert (Multitype.eq (mt₁ ⊎ {{ t ; mt₂}}) mt).
+    eq_multitype (union mt₁ mt₂) mt -> 
+    tight mt -> 
+    tight mt₁ /\ tight mt₂.
+Proof.
+  use_equivalences.
+  hint eq_tight_multitype.
+  inductions mt₁; intros; split_and_or; try solve[ simpls* ].
+  - change {{` t `; ` mt₁ `}} with (union {{t ; nil}} mt₁) in *.
+    asserts Heq : (eq_multitype (union mt₁ {{ t ; mt₂}}) mt).
     { 
-      change {{` t `; ` mt₂ `}} with (Multitype.union {{t ; nil}} mt₂) in *.
-      apply Multitype.eq_trans with ((mt₁ ⊎ {{t ; nil}}) ⊎ mt₂)...
-      - apply Multitype.eq_sym. apply Multitype.union_assoc.
-      - apply Multitype.eq_trans with (({{` t `; nil}} ⊎ mt₁) ⊎ mt₂)...
-        apply Multitype.eq_union_left.
-        apply Multitype.union_comm.
+      change {{` t `; ` mt₂ `}} with (union {{t ; nil}} mt₂) in *.
+      apply transitive with ((union (union mt₁ {{t ; nil}})) mt₂)...
+      - apply symmetric. apply union_assoc.
+      - apply transitive with (union (union {{` t `; nil}} mt₁) mt₂); autos.
+        apply eq_union_left;
+        apply union_comm.
     }
-    apply IHmt₁ in H1; repeat (split_and; simpl in *)...
+    apply IHmt₁ in Heq; repeat (split_and_or; simpls); autos.
+  - apply eq_tight_multitype 
+    with (mt₂ := union {{` t `; ` mt₁ `}} mt₂) in H0; 
+    simpls*; split_and_or_max.
+    edestruct IHmt₁; autos*.
 Qed.
 
 
-
-
-Lemma Ctx_union_tight : 
-  ∀ (Γ₁ Γ₂ Δ : Ctx.t), Γ₁ ⊎c Γ₂ ≡ Δ -> is_tight_context Δ -> is_tight_context Γ₁ /\ is_tight_context Γ₂.
-Proof with eauto using mt_union_tight, mt_union_tight, mt_eq_in, eq_tight, eq_tight_multitype with permutation_hints.
-  intros Γ₁ Γ₂ Δ.
-  generalize dependent Γ₂.
-  generalize dependent Γ₁.
-  induction Δ as [ | mt Δ IH]; intros * H_union H_tight; inversion H_union as [| Γ₁' Γ₂' H1 mt₁ mt₂ H2 H_union' H_eq H3 H4 H5 ]; subst; simpl in *; repeat split_and; try edestruct IH;
-  try destruct (mt_union_tight mt₁ mt₂ mt)...
+Lemma mt_tight_union :
+  ∀ mt₁ mt₂,
+  tight mt₁ ->
+  tight mt₂ ->
+  tight (mt₁ ⊎ mt₂).
+Proof.
+  induction mt₁; introv Htight1 Htight2; simpls*.
 Qed.
