Old/Context.v
@@ -1,0 +1,257 @@
+(* Require Import Tactics. *)
+Require Import Old.Types.
+From Coq Require Import Unicode.Utf8_core.
+
+From Coq Require Import List.
+Import ListNotations.
+
+Module Context (MT : MULTITYPE).
+  Definition t := list MT.T.
+
+  Inductive union : t -> t -> t -> Type :=
+  | Union_Nil : union [] [] [] 
+  | Union_Cons : 
+    ∀  Γ₁ Γ₂ Γᵣ mt₁ mt₂ mtu, 
+    union Γ₁ Γ₂ Γᵣ -> 
+    MT.eq (MT.union  mt₁ mt₂) mtu ->
+    union (mt₁ :: Γ₁) (mt₂ :: Γ₂) (mtu :: Γᵣ)
+  .
+  Hint Constructors union : core.
+
+  Fixpoint eq (Γ₁ Γ₂ : t) : Prop :=
+    match Γ₁, Γ₂ with 
+    | [], [] => True
+    | [], _::_ | _::_, [] => False
+    | h₁::t₁, h₂::t₂ => (MT.eq h₁ h₂) /\ (eq t₁ t₂)
+    end.
+  Hint Unfold eq : core.
+
+
+  Lemma eq_empty_l : ∀ Γ, eq [] Γ -> Γ = [].
+  Proof with eauto.
+    induction Γ; intros...
+    inversion H.
+  Qed.
+
+  Lemma eq_empty_r : ∀ Γ, eq Γ [] -> Γ = [].
+  Proof with eauto.
+    induction Γ; intros...
+    inversion H.
+  Qed.
+
+  Lemma eq_refl : ∀ Γ, eq Γ Γ.
+  Proof with eauto.
+    induction Γ; simpl...
+    split...
+    apply MT.eq_refl.
+  Qed.
+  
+
+  Lemma eq_sym : 
+    ∀ (Γ₁ Γ₂ : t),
+    eq Γ₁ Γ₂ ->
+    eq Γ₂ Γ₁.
+  Proof with eauto.
+    induction Γ₁ as [| mt₁ Γ₁]; intros [| mt₂ Γ₂ ] H_eq; simpl in *; repeat split_and...
+    apply MT.eq_sym...
+  Qed.
+
+
+  Lemma eq_trans : 
+    ∀ (Γ₁ Γ₂ Γ₃: t),
+    eq Γ₁ Γ₂ ->
+    eq Γ₂ Γ₃ ->
+    eq Γ₁ Γ₃.
+  Proof with eauto.
+    induction Γ₁ as [| mt₁ Γ₁]; intros [| mt₂ Γ₂ ] [| mt₃ Γ₃ ] H_eq1 H_eq2; simpl in *; repeat split_and; try contradiction...
+    eapply MT.eq_trans...
+  Qed.
+
+  Theorem union_comm : 
+    ∀ (Γ₁ Γ₂ Γᵣ₁ Γᵣ₂: t),
+    union Γ₁ Γ₂ Γᵣ₁ -> 
+    union Γ₂ Γ₁ Γᵣ₂ -> 
+    eq Γᵣ₁ Γᵣ₂.
+  Proof with eauto.
+    intros * H_union_1. generalize dependent Γᵣ₂.
+    induction H_union_1; intros * H_union_2; inversion H_union_2; subst; simpl...
+    split...
+    eapply MT.eq_trans...
+    apply MT.eq_sym.
+    apply MT.eq_trans with (MT.union mt₁ mt₂)...
+    apply MT.union_comm.
+  Qed.
+
+  Ltac inversion_eq_list := 
+    match goal with 
+    | [H : _ :: _ = _ :: _ |- _] => inversion H; clear H; subst
+    end.
+
+  Theorem union_assoc : 
+    ∀ (Γ₁ Γ₂ Γ₃ Γ₁₂ Γ₁₂_₃ Γ₂₃ Γ₁_₂₃ : t),
+    union Γ₁ Γ₂ Γ₁₂ -> 
+    union Γ₁₂ Γ₃ Γ₁₂_₃ -> 
+    union Γ₂ Γ₃ Γ₂₃ -> 
+    union Γ₁ Γ₂₃ Γ₁_₂₃ -> 
+    eq Γ₁₂_₃ Γ₁_₂₃.
+  Proof with eauto using MT.eq_refl, MT.eq_sym, MT.eq_trans, MT.union_assoc, MT.eq_union.
+  Hint Unfold eq : core.
+  intros * H_union_1_2.
+  generalize dependent Γ₃.
+  generalize dependent Γ₁₂_₃. 
+  generalize dependent Γ₂₃.
+  generalize dependent Γ₁_₂₃.
+  induction H_union_1_2; intros * H_union_12_3 H_union_2_3 H_union_1_23; inversion H_union_12_3; inversion H_union_2_3; inversion H_union_1_23; subst...
+  simpl.
+  repeat inversion_eq_list.
+  (* inversion H8; inversion H14; subst. *)
+  split...
+  apply MT.eq_trans with (MT.union mt₁ mtu1)...
+  apply MT.eq_trans with (MT.union mtu mt₂0)...
+  apply MT.eq_trans with (MT.union mt₁ (MT.union mt₂ mt₂0))...
+Qed.
+
+
+
+  Lemma eq_union_left : 
+    ∀ Γ₁ Γ₁' Γ₂ Γᵣ, 
+    eq Γ₁ Γ₁'-> 
+    union Γ₁ Γ₂ Γᵣ -> 
+    union Γ₁' Γ₂ Γᵣ
+    .
+  Proof with eauto 6 using MT.eq_union, MT.eq_sym, MT.eq_refl, MT.eq_trans, Union_Cons with permutation_hints.
+    induction Γ₁ as [ | mt₁ Γ₁ IHΓ]; intros [| mt₁' Γ₁'] [ | mt₂ Γ₂] [| mtᵣ Γᵣ] H_eq H_u; inversion H_u; try inversion H_eq; subst; simpl...
+  Qed.
+
+  Lemma eq_union_right : 
+    ∀ Γ₁ Γ₂ Γ₂' Γᵣ, 
+    eq Γ₂ Γ₂'-> 
+    union Γ₁ Γ₂ Γᵣ -> 
+    union Γ₁ Γ₂' Γᵣ
+    .
+  Proof with eauto 6 using MT.eq_union, MT.eq_sym, MT.eq_refl, MT.eq_trans, Union_Cons with permutation_hints.
+    induction Γ₁ as [ | mt₁ Γ₁ IHΓ]; intros [| mt₂ Γ₂] [ | mt₂' Γ₂'] [| mtᵣ Γᵣ] H_eq H_u; inversion H_u; try inversion H_eq; subst; simpl...
+  Qed.
+
+  Lemma eq_union : 
+    ∀ Γ₁ Γ₁' Γ₂ Γ₂' Γᵣ, 
+    eq Γ₁ Γ₁'-> 
+    eq Γ₂ Γ₂'-> 
+    union Γ₁ Γ₂ Γᵣ -> 
+    union Γ₁' Γ₂' Γᵣ.
+  Proof.
+    eauto using eq_trans, eq_union_left, eq_union_right with permutation_hints.
+  Qed.    
+
+End Context.
+
+Module Ctx := Context Multitype.
+
+
+Fixpoint is_tight_context(Γ : Ctx.t) : Prop :=
+  match Γ with 
+  | [] => True 
+  | h::t => (is_tight_multitype h) /\ (is_tight_context t) 
+  end.
+
+
+Hint Unfold is_tight_type is_tight_multitype is_tight_context  : core.
+Notation "a ⊎ b" := (Multitype.union a b) (at level 0).
+Notation "a '⊎c' b ≡ c" := (Ctx.union a b c) (at level 0).
+
+
+
+Fixpoint In (t : type) (mt : multitype) : Prop :=
+  match mt with 
+  | {{ nil }} => False
+  | {{ h ; mt }} => (permutationₜ t h) \/ (In t mt)
+  end.
+
+Lemma mt_eq_in : 
+  ∀ (t : type) (mt₁ mt₂ : multitype),
+  Multitype.eq mt₁ mt₂ -> 
+  In t mt₁ ->
+  In t mt₂.
+Proof with eauto with permutation_hints.
+  intros * H_eq H_in.
+  induction H_eq...
+  - inversion H_in.
+    + left...
+    + right...
+  - inversion H_in.
+    + right. left...
+    + inversion H.
+      * left...
+      * right; right...
+Qed.
+
+
+Ltac permutationₜ_induction perm P0 := 
+  induction perm using permutationₜ_mut_ind with (P0:=P0); unfold P0 in *; clear P0.
+
+Ltac permutationₘ_induction perm P := 
+  induction perm using permutationₘ_mut_ind with (P:=P); unfold P in *; clear P.
+
+Lemma eq_tight : 
+  ∀ t₁ t₂, 
+  permutationₜ t₁ t₂ ->
+  is_tight_type t₁ -> 
+  is_tight_type t₂.
+Proof with eauto using mt_eq_in with permutation_hints.
+  intros * H_perm.
+  pose (P0 (mt₁ mt₂ : multitype) (H_permₘ : permutationₘ mt₁ mt₂) := is_tight_multitype mt₁ -> is_tight_multitype mt₂).
+  permutationₜ_induction H_perm P0; try (intro H_tight; split; inversion H_tight as [H_tight_t H_tight_mt]; try inversion H_tight_mt; eauto using mt_eq_in with permutation_hints; fail)...
+Qed.
+
+Lemma eq_tight_multitype : 
+  ∀ mt₁ mt₂, 
+  permutationₘ mt₁ mt₂ ->
+  is_tight_multitype mt₁ -> 
+  is_tight_multitype mt₂.
+Proof with eauto using mt_eq_in with permutation_hints.
+  intros * H_perm.
+  pose (P (t₁ t₂ : type) (H_permₜ : permutationₜ t₁ t₂) := is_tight_type t₁ -> is_tight_type t₂).
+  permutationₘ_induction H_perm P; try (intro H_tight; split; inversion H_tight as [H_tight_t H_tight_mt]; try inversion H_tight_mt; repeat apply and_set_intro; eauto using mt_eq_in with permutation_hints; fail)...
+Qed.
+
+
+Lemma Ctx_eq_tight :
+  ∀ (Γ₁ Γ₂ : Ctx.t), Ctx.eq Γ₁ Γ₂ -> is_tight_context Γ₁ -> is_tight_context Γ₂.
+Proof with eauto using mt_eq_in, eq_tight, eq_tight_multitype with permutation_hints.
+  induction Γ₁; intros; destruct Γ₂; simpl in *; destruct H, H0...
+Qed.
+
+
+Lemma mt_union_tight :
+  ∀ (mt₁ mt₂ mt : multitype), 
+    Multitype.eq (mt₁ ⊎ mt₂) mt -> 
+    is_tight_multitype mt -> 
+    is_tight_multitype mt₁ /\ is_tight_multitype mt₂.
+Proof with eauto using mt_eq_in, eq_tight, eq_tight_multitype with permutation_hints.
+  induction mt₁; intros; simpl.
+  - split...
+  - change {{` t `; ` mt₁ `}} with (Multitype.union {{t ; nil}} mt₁) in *.
+    assert (Multitype.eq (mt₁ ⊎ {{ t ; mt₂}}) mt).
+    { 
+      change {{` t `; ` mt₂ `}} with (Multitype.union {{t ; nil}} mt₂) in *.
+      apply Multitype.eq_trans with ((mt₁ ⊎ {{t ; nil}}) ⊎ mt₂)...
+      - apply Multitype.eq_sym. apply Multitype.union_assoc.
+      - apply Multitype.eq_trans with (({{` t `; nil}} ⊎ mt₁) ⊎ mt₂)...
+        apply Multitype.eq_union_left.
+        apply Multitype.union_comm.
+    }
+    apply IHmt₁ in H1; repeat (split_and; simpl in *)...
+Qed.
+
+
+
+
+Lemma Ctx_union_tight : 
+  ∀ (Γ₁ Γ₂ Δ : Ctx.t), Γ₁ ⊎c Γ₂ ≡ Δ -> is_tight_context Δ -> is_tight_context Γ₁ /\ is_tight_context Γ₂.
+Proof with eauto using mt_union_tight, mt_union_tight, mt_eq_in, eq_tight, eq_tight_multitype with permutation_hints.
+  intros Γ₁ Γ₂ Δ.
+  generalize dependent Γ₂.
+  generalize dependent Γ₁.
+  induction Δ as [ | mt Δ IH]; intros * H_union H_tight; inversion H_union as [| Γ₁' Γ₂' H1 mt₁ mt₂ H2 H_union' H_eq H3 H4 H5 ]; subst; simpl in *; repeat split_and; try edestruct IH;
+  try destruct (mt_union_tight mt₁ mt₂ mt)...
+Qed.
