Old/HeadEvaluation.v
@@ -1,0 +1,539 @@
+(*
+  Tight Typings and Split Bounds,
+    BENIAMINO ACCATTOLI
+    STÉPHANE GRAHAM-LENGRAND
+    DELIA KESNER
+  https://arxiv.org/pdf/1807.02358.pdf
+*)
+Set Default Goal Selector "!".
+From Coq Require Import String.
+From Coq Require Import PeanoNat.
+From Coq Require Import Arith.
+From Coq Require Import Unicode.Utf8.
+From Coq Require Import Lia.
+From Coq Require Import Lists.ListSet.
+From Coq Require Import List.
+From Coq Require Import Classes.Equivalence.
+Require Import EvaluationSystem.
+Require Import Old.Tactics.
+Require Import Syntax.
+Require Import Old.Types.
+Require Import Old.Context.
+Import ListNotations.
+
+
+
+Inductive neutral : term -> Prop :=
+| Neutral_Var : ∀ (n : nat), neutral <{#n}>
+| Neutral_App : ∀ (t₁ t₂ : term), neutral t₁ -> neutral <{t₁ t₂}>
+.
+Inductive normal : term -> Prop := 
+| Normal_Neutral : ∀ (t : term), neutral t -> normal t 
+| Normal_Abs : ∀ (t : term), normal t -> normal <{λ t}> 
+.
+Hint Constructors neutral : core.
+Hint Constructors normal : core.
+
+Ltac neutral_to_normal t := 
+  match goal with 
+  | [H : neutral t |- _] => let H_normal := fresh "H_normal" in apply Normal_Neutral in H 
+  end.  
+
+Inductive abs : term -> Prop := 
+| Abs : ∀ (t : term), abs <{ λ t }>
+.
+Hint Constructors abs : core.
+
+Hint Extern 1 =>
+  match goal with 
+  | [H : abs (Trm_Bound_Var _) |- _] => inversion H
+  | [H : abs (Trm_App _ _) |- _] => inversion H
+  | [H : ¬ abs (Trm_Abs _) |- _] => exfalso; apply H; apply Abs
+  | [H : neutral (Trm_Abs _) |- _] => inversion H 
+  end : core.
+
+Hint Extern 1 (¬ neutral (Trm_Abs _)) =>
+  let H := fresh in 
+  intro H;
+  inversion H 
+: core.
+
+
+Hint Extern 1 (¬ abs (Trm_App _ _)) => 
+  let H := fresh in 
+  intro H;
+  inversion H 
+ : core.
+
+Hint Extern 1 (¬ abs (Trm_Bound_Var _)) => 
+  let H := fresh in 
+  intro H;
+  inversion H 
+ : core.
+
+Reserved Notation "a --> b" (at level 0).
+Inductive step : term -> term -> Prop :=
+| ST_Beta : 
+    ∀ (u q : term), 
+    <{ (λ u) q }> --> (lower 0 <{u[0 <- q]}>)
+| ST_Abs : 
+    ∀ (t p : term),
+    t --> p -> 
+    <{λ t}> --> <{λ p}>
+| ST_App : 
+    ∀ (t p u : term), 
+    (¬ abs t) -> 
+    t --> p ->
+    <{t u}> --> <{p u}>
+where 
+  "a --> b" := (step a b)
+.
+Hint Constructors step : core.
+
+Theorem deterministic_step : deterministic step.
+Proof with (myauto idtac).
+  unfold deterministic.
+  intros * H.
+  generalize dependent a₂.
+  induction H; intros;
+  match goal with 
+  | [H : step _ _ |- _] => 
+      inversion H; subst; 
+      f_equal || exfalso; auto
+  end. 
+Qed.
+Hint Resolve deterministic_step : core.
+
+
+Definition multistep : term -> term -> Set := reflexive_closure (transitive_closure step).
+Notation "a -->* b" := (multistep a b) (at level 0).
+
+Fixpoint size (t : term) : nat := 
+  match t with
+  | <{ #_ }> => 0 
+  | <{λ t}> 
+  | <{ t _ }> => 1 + size t
+  end.
+
+Hint Unfold size  : HeadEvaluation.
+
+
+
+Goal <{(λ λ #1 #2) (λ #0)}> --> <{λ (λ #0) #1}>.
+apply ST_Beta.
+Qed.
+
+
+Hint Extern 1 => 
+  match goal with 
+  | [H : <{#_}> --> _ |- _] => inversion H 
+  end 
+: core.
+
+Lemma neutral_is_normal_not_abs : 
+  ∀ (t : term), 
+  normal t -> (¬ abs t) -> 
+  neutral t.
+Proof with auto.
+  intros * H_normal_t H_not_abs_t.
+  inversion H_normal_t; subst...
+Qed.
+Hint Resolve neutral_is_normal_not_abs : core.
+
+
+Ltac destruct_hyp :=
+  repeat match goal with 
+  | [H : _ /\ _ |- _] => destruct H 
+  | [H : ∃ _, _ |- _] => destruct H 
+  | [H : ¬ _ |- _] => unfold not in H 
+  end.  
+
+
+Ltac intros_destruct :=
+unfold not; 
+intros; destruct_hyp.
+
+Theorem head_red_eval_system :
+  evaluation_system term step normal neutral abs.
+Proof with repeat intros_destruct; try (exfalso; eauto; fail); eauto.
+  repeat split...
+  - unfold rel_normal in *.
+    induction t...
+    + induction t1...
+      apply Normal_Neutral. apply Neutral_App. 
+      apply neutral_is_normal_not_abs...
+      apply IHt1...
+    + apply Normal_Abs. apply IHt...
+  - intro.
+    induction H as [t H_neutral | t H_norm IH].
+    + induction H_neutral...
+      inversion H; subst...
+    + apply IH... inversion H; subst... 
+  - inversion H; subst...
+Qed.
+
+
+
+Section HeadTypingSystem.
+
+        (* TODO:
+          Rajouter multi-ensemble vide 
+          ou 
+          remplacer singleton par vide + T_Many: un multitype et un type *)
+        
+
+    Reserved Notation "Γ '|(' b ',' r ')-' t '∈' T" (at level 70).
+    Reserved Notation "Γ '|(' b ',' r ')-' t '∈ₘ' T" (at level 70).
+
+    Inductive has_type : Ctx.t -> nat -> nat -> term -> type -> Type :=
+    | T_Ax0 :
+        ∀ {A : type},
+        [ {{ A ; nil }} ] |(0, 0)- <{ #0 }> ∈ A
+    | T_Ax0_Empty : 
+        ∀ {A: type} {h : multitype} {Γ : Ctx.t},
+        h::Γ |(0, 0)- <{#0}> ∈ A ->
+        h::{{nil}}::Γ |(0, 0)- <{#0}> ∈ A
+    | T_AxS : 
+        ∀ {A: type} {Γ : Ctx.t} {x : nat},
+        Γ |(0, 0)- <{#x}> ∈ A ->
+        {{nil}}::Γ |(0, 0)- <{#`S x`}> ∈ A
+    
+    | T_Fun_b :
+        ∀ {t : term} {mt : multitype} {A : type} {Γ : Ctx.t} {b r : nat},
+        mt :: Γ |(b, r)- t ∈ A -> 
+        Γ |(S b, r)- <{ λ t }> ∈ Ty_Fun mt A
+    | T_Fun_r : 
+        ∀ {t : term} {T A : type} {Γ : Ctx.t} {b r : nat},
+        is_tight_type A ->
+        is_tight_type T ->
+        (MT_Cons T MT_Empty) :: Γ |(b, r)- t ∈ A -> 
+        Γ |(b, S r)-  <{ λ t }> ∈ Ty_Tight TC_Abs 
+    | T_App_b :
+        ∀ {Γ₁ Γ₂ Δ : Ctx.t} {M : multitype} {A : type}
+          {b₁ b₂ r₁ r₂ : nat} {t₁ t₂ : term}, 
+        Γ₁ ⊎c Γ₂ ≡ Δ ->
+        Γ₁ |(b₁, r₁)- t₁ ∈ Ty_Fun M A ->
+        Γ₂ |(b₂, r₂)- t₂ ∈ₘ M ->  
+        Δ |(b₁ + b₂, r₁ + r₂)- <{ t₁ t₂ }> ∈ A
+    | T_App_hd_r :
+        ∀ {Γ : Ctx.t} {t₁ t₂ : term} {b r : nat},
+        Γ |(b, r)- t₁ ∈ Ty_Tight TC_Neutral -> 
+        Γ |(b, S r)- <{ t₁ t₂ }> ∈ Ty_Tight TC_Neutral
+    where 
+      "Γ '|(' b ',' r ')-' t '∈' T" := (has_type Γ b r t T)
+    with has_many_types : Ctx.t -> nat -> nat -> term -> multitype -> Type :=
+    | ManyT_Empty : [] |(0, 0)- <{#0}> ∈ₘ {{nil}}
+    | ManyT_Singleton :
+      ∀ {Γ : Ctx.t} {t : term} {A : type} {b r : nat},
+        Γ |(b, r)- t ∈ A ->
+        Γ |(b, r)- t ∈ₘ {{ A ; nil }} 
+    | ManyT_Union :
+        ∀ {Γ₁ Γ₂ Δ: Ctx.t} {t : term} {A : type} {mt : multitype} {b₁ b₂ r₁ r₂ : nat},
+        Γ₁ ⊎c Γ₂ ≡ Δ ->
+        Γ₁ |(b₁, r₁)- t ∈ₘ mt ->
+        Γ₂ |(b₂, r₂)- t ∈ A ->
+        Δ |(b₁ + b₂, r₁ + r₂)- t ∈ₘ {{A; mt}}
+    | ManyT_Inv :
+      ∀ {Γ₁ Γ₂ Δ : Ctx.t} {t : term} {A : type} {mt : multitype} {b₁ b₂ r₁ r₂ : nat},
+        Γ₁ ⊎c Γ₂ ≡ Δ ->
+        (* Multitype.eq (mt₁ ⊎ mt₂) mtᵤ -> *)
+        Δ  |(b₁ + b₂, r₁ + r₂)- t ∈ₘ {{A; mt}} ->
+        Γ₁ |(b₁, r₁)- t ∈ A ->
+        Γ₂ |(b₂, r₂)- t ∈ₘ mt
+
+    where 
+      "Γ '|(' b ',' r ')-' t '∈ₘ' T" := (has_many_types Γ b r t T)
+    .
+
+
+
+    Lemma TAx_is_0_many : 
+      ∀ {Γ: Ctx.t} {n : nat} {b r : nat},
+      Γ |(b, r)- <{#n}> ∈ₘ {{ nil }} ->
+      b = 0 /\ r = 0.
+    Proof with eauto.
+      intros Γ n.
+      generalize dependent Γ.
+      induction n; intros * φ.
+      - inversion φ; subst... admit.
+      - destruct Γ; try destruct t; inversion φ; subst...
+        Admitted.
+    (* Qed. *)
+
+    Lemma TAx_is_0 : 
+      ∀ {Γ: Ctx.t} {n : nat} {A : type} {b r : nat},
+      Γ |(b, r)- <{#n}> ∈ A ->
+      b = 0 /\ r = 0.
+    Proof with eauto.
+      intros Γ n.
+      generalize dependent Γ.
+      induction n; intros * φ.
+      - inversion φ...
+      - destruct Γ; try destruct t; inversion φ...
+    Qed.
+    Lemma T_Many_Inv :
+        ∀ {Γ: Ctx.t} {t : term} {A : type} {b r : nat},
+        Γ |(b, r)- t ∈ₘ {{A ; nil}} -> 
+        Γ |(b, r)- t ∈ A.
+    Proof with eauto.
+      intros Γ t.
+      generalize dependent Γ.
+      induction t; intros * φ; inversion φ; subst...
+      - apply TAx_is_0 in H7 as [-> ->]. admit.
+      (* - inversion HeqM.
+      - inversion HeqM; subst...
+      - inversion HeqM; subst... admit. *)
+      - subst.  
+    Admitted.
+
+    Hint Constructors has_type has_many_types : core.
+    Scheme has_type_mut_ind := Induction for has_type Sort Type
+    with has_many_types_mut_ind := Induction for has_many_types Sort Type.
+    Scheme has_type_mut_rec := Induction for has_type Sort Set
+    with has_many_types_mut_rec := Induction for has_many_types Sort Set.
+
+  
+
+
+  Fixpoint size_typing_derivation {b r : nat} {Γ : Ctx.t} {t : term} {T : type} (der : Γ |( b , r )- t ∈ T) : nat :=
+    match der with 
+      | T_Ax0  => 0
+      | T_Ax0_Empty _ => 0
+      | T_AxS _  => 0
+      (* | T_Many_Inv der => size_many_typing_derivation der *)
+      | T_Fun_b der' => S (size_typing_derivation der')
+      | T_Fun_r _ _ der' => S (size_typing_derivation der')
+      | T_App_b _ der₁ der₂ => 
+          S ((size_typing_derivation der₁) + (size_many_typing_derivation der₂))
+      | T_App_hd_r der' => S (size_typing_derivation der')
+      end
+  with
+    size_many_typing_derivation {b r : nat} {Γ : Ctx.t} {t : term} {M : multitype} (der : Γ |( b , r )- t ∈ₘ M) : nat :=
+    match der with 
+    | ManyT_Empty => 0
+    | ManyT_Singleton der => size_typing_derivation der
+    | ManyT_Union _ der₁ der₂ => size_many_typing_derivation der₁ + size_typing_derivation der₂
+    | ManyT_Inv _ mder der =>size_many_typing_derivation mder +  size_typing_derivation der
+    end
+  .
+
+  Definition is_tight_derivation 
+    {b r : nat} {Γ : Ctx.t} {t : term} {T : type} 
+    (der : Γ |( b , r )- t ∈ T) : Prop 
+  := 
+    (is_tight_type T) /\  (is_tight_context Γ).
+    
+    Check has_type_mut_ind.
+
+Ltac derivation_induction der P0 := 
+  induction der using has_type_mut_ind with (P0:=P0); unfold P0 in *; clear P0.
+
+        
+Goal ∀ {Γ: Ctx.t} {t : term} {A : type} {b r : nat} (φ : Γ |(b, r)- t ∈ A),
+  b + r <= size_typing_derivation φ.
+  Proof.
+    intros.
+    pose (P0 (Γ: Ctx.t) (b r : nat) (t : term) (M : multitype) (φ : Γ |(b, r)- t ∈ₘ M) := b + r <= size_many_typing_derivation φ).
+    derivation_induction φ P0; simpl; lia.
+  Qed.
+
+Definition Id := <{ λ #0 }>.
+Definition example_term := <{ (λ ((λ #0 #1) #0)) `Id` }>.
+Example example_1_is_Id : example_term -->* Id.
+Proof.
+  unfold example_term.
+  apply RC_self.
+  eapply TC_trans.
+  - eapply TC_self. apply ST_Beta.
+  - simpl. eapply TC_trans; simpl; eapply TC_self.
+    + eapply ST_Beta. 
+    + eapply ST_Beta.
+Qed. 
+
+Definition abs_abs := {{ ` Ty_Tight TC_Abs ` ; nil }} |-> Ty_Tight TC_Abs.
+
+Example first_derivation : [] |(3, 1)- example_term ∈ (Ty_Tight TC_Abs).
+Proof with eauto using Ctx.Union_Nil, Ctx.Union_Cons, Multitype.eq_refl.
+  unfold example_term.
+  apply @T_App_b with 
+    (b₁ := 2)
+    (b₂ := 1)
+    (r₁ := 0)
+    (r₂ := 1)
+    (Γ₁ := []) 
+    (Γ₂ :=[]) 
+    (
+    M := {{ 
+        ` Ty_Tight TC_Abs ` ; 
+        ` abs_abs ` ; 
+          nil 
+        }}
+    )...
+  - apply T_Fun_b.
+    apply @T_App_b with 
+      (Γ₁ := [{{ ` Ty_Tight TC_Abs ` ; nil }}]) 
+      (Γ₂ := [{{ ` abs_abs ` ; nil }}]) 
+      (b₁ := 1) 
+      (b₂ := 0) 
+      (r₁ := 0) 
+      (r₂ := 0)
+       (M := {{ abs_abs ; nil}})...
+    apply T_Fun_b.
+    unfold abs_abs.
+    apply @T_App_b with 
+    (Γ₁ := [ {{ ` abs_abs ` ; nil }} ; {{nil}}])
+    (Γ₂ := [ {{nil}}; {{ ` Ty_Tight TC_Abs ` ; nil }} ])
+    (b₁ := 0) (b₂ := 0) (r₁ := 0) (r₂ := 0) (M := {{ ` Ty_Tight TC_Abs ` ; nil }}); unfold abs_abs...
+  - unfold Id.
+    change 1 with (1 + 0) at 1.
+    change 1 with (0 + 1) at 2.
+    eapply @ManyT_Union with (A := Ty_Tight TC_Abs) (mt := {{ `abs_abs` ; nil }}); unfold abs_abs...
+    eapply @T_Fun_r
+      with (T := Ty_Tight TC_Abs) (A := Ty_Tight TC_Abs)...
+Qed.
+
+
+
+Definition last_rule_is_appb 
+    {b r : nat} {Γ : Ctx.t} {t : term} {T : type} 
+    (der : Γ |( b , r )- t ∈ T) : Prop := 
+  match der with 
+  | T_Ax0 => False
+  | T_Ax0_Empty _ => False
+  | T_AxS _ => False
+  | T_Fun_b _ => False
+  | T_Fun_r _ _ _ => False
+  | T_App_b _ _ _ => True
+  | T_App_hd_r _ => False
+  end.
+
+
+Lemma tight_spreading_var :  
+  ∀ {Γ : Ctx.t} {b r : nat} {x : nat} {A : type}
+    (φ : Γ |( b, r )- Trm_Bound_Var x ∈ A), 
+  is_tight_context Γ -> 
+  is_tight_type A /\ ¬ last_rule_is_appb φ.
+Proof with eauto.
+  intros * H_tight.
+  split.
+  + generalize dependent Γ.
+    generalize dependent b. 
+    generalize dependent r. 
+    generalize dependent A. 
+    induction x; intros * φ H_tight.
+    - remember (Trm_Bound_Var 0) as t.
+      induction φ; subst; simpl in *; destruct_hyp;
+      try (inversion Heqt; fail)...
+    - remember (Trm_Bound_Var (S x)) as t. 
+      induction φ; subst; simpl in *; destruct_hyp;
+      inversion Heqt; subst...
+  + intros * H_contra.
+    remember (Trm_Bound_Var x) as t.
+    destruct φ eqn:H_eq...
+    inversion Heqt. 
+Qed.
+
+Ltac tight_union Δ :=
+  match goal with 
+  | [H : ?Γ₁ ⊎c ?Γ₂ ≡ Δ |- _] => 
+    let H_tight_Γ₁ := fresh "H_tight_Γ₁" in 
+    let H_tight_Γ₂ := fresh "H_tight_Γ₂" in 
+      apply Ctx_union_tight in H as  [H_tight_Γ₁ H_tight_Γ₂]; eauto 
+  end.
+
+
+
+Lemma tigh_spreading_on_neutral_terms : 
+  ∀ {t : term}, neutral t ->
+  ∀ {Γ : Ctx.t} {b r : nat} {A : type}
+    (φ : Γ |(b, r)- t ∈ A), 
+  is_tight_context Γ ->
+  is_tight_type A /\ ¬ last_rule_is_appb φ.
+Proof with eauto.
+  intros t H_neutral.
+  induction H_neutral as [ x | p u H_neutral_p IH]; intros Γ b r A φ H_tight.
+  - eapply tight_spreading_var...
+  - inversion φ; subst...
+    + tight_union Γ.
+      apply IH in H5; simpl in H5; try contradiction...
+    + split...
+      remember <{ ` p ` ` u ` }> as t.
+      remember (Ty_Tight TC_Neutral) as T.
+      destruct φ eqn:Heq; simpl; inversion Heqt; subst...
+      tight_union Δ.
+      apply IH with (φ := h) in H_tight_Γ₁ as [H_contra _]; simpl in *; contradiction.
+Qed.
+
+
+Lemma normal_size_derivation : 
+  ∀ {t : term} {Γ : Ctx.t} {b r : nat} {A : type} 
+    (φ : Γ |(b, r)- t ∈ A), 
+  normal t -> 
+  size t <= size_typing_derivation φ.
+Proof with try lia.
+  intros * H_normal_t.
+  induction φ; inversion H_normal_t; subst; simpl; try apply IHφ in H0; 
+  try (
+    inversion H; subst;
+    neutral_to_normal t₁;
+    apply IHφ in H1; lia
+  )...
+Qed.
+
+Ltac use_type_spreading Γ :=
+  match goal with 
+  | [ H : Γ |(_, _)- _ ∈ {{ {{_}} |-> _}} |- _] => 
+      apply tigh_spreading_on_neutral_terms in H; eauto; subst; inversion H
+  end. 
+
+Theorem normal_tight_der_size_b_r :
+  ∀ {t : term} {Γ : Ctx.t} {b r : nat} {A : type} 
+    (φ : Γ |(b, r)- t ∈ A), 
+  normal t -> 
+  is_tight_derivation φ -> 
+  b = 0 /\ r = size t.
+Proof with try lia; eauto using Ctx_union_tight.
+  induction t; intros * H_normal_t H_tight_der; destruct H_tight_der as [H_tight_A H_tight_Γ]; inversion φ; subst; simpl; try (inversion H_tight_A; fail)...
+  - assert (is_tight_context Γ₁ /\ is_tight_context Γ₂) 
+      as [H_tight_Γ₁ H_tight_Γ₂]...
+    inversion H_normal_t. inversion H; subst.
+    use_type_spreading Γ₁.
+  - inversion H_normal_t; inversion H; subst.
+    apply Normal_Neutral in H2.
+    eapply IHt1 with (φ := H5) in H2; try split...
+  - inversion H_normal_t; subst; 
+    destruct (IHt _ _ _ _ H5); try split...
+Qed.  
+
+Theorem normal_neutral_type_is_neutral : 
+  ∀ {t : term} {Γ : Ctx.t} {b r : nat} 
+    (φ : Γ |(b, r)- t ∈ Ty_Tight TC_Neutral), 
+  normal t -> 
+  neutral t.
+Proof with eauto.
+  induction t; intros * φ H_normal_t; inversion H_normal_t; inversion φ...
+Qed.
+
+
+Lemma substitution_typing :
+  ∀ 
+    (Γ₁ Γ₂ Δ : Ctx.t) (H_u : Γ₁ ⊎c Γ₂ ≡ Δ) (M : multitype) 
+    (b r b' r' : nat) (t p : term) (A : type) 
+    (φₜ : M :: Γ₁ |(b, r)- t ∈ A) (φₚ : Γ₂ |(b', r')- p ∈ₘ M),
+    Δ |(b + b', r + r')- lower 0 <{t[0 <- p]}> ∈ A
+    (* ∃ (φ : Δ |(b + b', r + r')- lower 0 <{t[0 <- p]}> ∈ A),
+    size_typing_derivation φ = size_many_typing_derivation φₚ + size_typing_derivation φₜ - Multitype.size M *)
+  .
+Proof with eauto with arith.
+  intros.
+  induction φₜ eqn:Heqt.
+  - induction φₚ eqn:Heqp; simpl.
+    + admit.  
+    + admit.
+    + destruct t; simpl. 
+      * destruct n; simpl.
+  
+Admitted.
+End HeadTypingSystem.
+
+
