Old/Tactics.v
@@ -1,0 +1,19 @@
+
+Ltac absurd := 
+  let H := fresh in
+  intro H; inversion H; fail.
+
+Ltac myauto t := 
+               (absurd; fail) 
+            || (exfalso; eauto; fail)
+            || (t; fail)
+            || eauto.
+
+Tactic Notation "'myauto'" := myauto idtac.
+
+
+Ltac split_and := 
+  match goal with 
+  | [ |- _ /\ _ ] => split
+  | [H : _ /\ _ |- _] => destruct H
+  end.
