theories/Classes.v
@@ -1,0 +1,30 @@
+From TLC Require Import LibRelation.
+From Coq Require Import Unicode.Utf8_core.
+
+Class Equivalence {A : Type} (relation : A -> A -> Type) : Type :=
+  { 
+    reflexive : 
+      ∀ a, 
+      relation a a
+
+  ; symmetric : 
+      ∀ a₁ a₂, 
+      relation a₁ a₂ -> 
+      relation a₂ a₁ 
+
+  ; transitive : 
+      ∀ a₁ a₂ a₃, 
+      relation a₁ a₂ -> 
+      relation a₂ a₃ -> 
+      relation a₁ a₃ 
+  }.
+
+Class Tightable (A : Type) : Type := 
+  { tight : A -> Prop }.
+
+Class Sized (A : Type) : Type := 
+  { size : A -> nat }.
+
+
+
+
