theories/Context.v
@@ -1,0 +1,221 @@
+
+From TLC Require Import LibLN LibTactics LibFset.
+From Coq Require Import Unicode.Utf8_core.
+From TTSB Require Import Types.
+
+Definition ctx : Type := vars * (var -> multitype).
+Definition empty : ctx := (\{}, fun _ => {{nil}}).
+Definition add (Γ : ctx) (v : var) (e : multitype) : ctx :=
+  If e = MT_Empty 
+  then Γ 
+  else
+    let (s, f) := Γ in 
+    (s \u \{v}, fun x => If x = v then e ⊎ (f x) else f x).
+
+
+Definition union_ctx (Γ₁ Γ₂ : ctx) : ctx :=
+  let (s₁, f₁) := Γ₁ in
+  let (s₂, f₂) := Γ₂ in
+  (s₁ \u s₂, fun x => (f₁ x) ⊎ (f₂ x)).
+
+
+
+Notation "a '⊎c' b"  := (union_ctx a b) (at level 0).
+Definition eq_ctx (Γ₁ Γ₂ : ctx) : Prop :=
+  let (s₁, f₁) := Γ₁ in
+  let (s₂, f₂) := Γ₂ in
+  s₁ = s₂ /\ 
+  ∀ (x : var),  
+  Multitype.eq (f₁ x) (f₂ x).
+
+
+Lemma eq_refl : 
+  ∀ Γ, eq_ctx Γ Γ.
+Proof.
+  Hint Resolve Multitype.eq_refl : core.
+  destruct Γ; simpls*.
+Qed.
+
+Lemma eq_sym : 
+  ∀ Γ₁ Γ₂, eq_ctx Γ₁ Γ₂ -> eq_ctx Γ₂ Γ₁.
+Proof.
+  Hint Resolve Multitype.eq_sym : core.
+  introv H_eq;
+  destruct Γ₁ eqn:Heq₁; destruct Γ₂ eqn:Heq₂; splits*;
+  inverts* H_eq. 
+Qed.
+
+Lemma eq_trans : 
+  ∀ Γ₁ Γ₂ Γ₃, eq_ctx Γ₁ Γ₂ -> eq_ctx Γ₂ Γ₃ -> eq_ctx Γ₁ Γ₃.
+Proof.
+  Hint Resolve Multitype.eq_trans : core.
+  intros [s₁ f₁] [s₂ f₂] [s₃ f₃] H_eq1 H_eq2; splits;
+  inverts H_eq1; inverts* H_eq2. 
+Qed.
+
+Lemma union_empty_l :
+  ∀ Γ, eq_ctx (empty ⊎c Γ) Γ.
+Proof.
+  intros [s f].
+  simpls.
+  splits*;
+  rewrite* LibFset.union_empty_l.
+Qed.
+
+Lemma union_empty_r :
+  ∀ Γ, eq_ctx (Γ ⊎c empty) Γ.
+Proof.
+  Hint Resolve Multitype.union_empty_r : core.
+  intros [s f].
+  simpls;
+  splits;
+  try rewrite* LibFset.union_empty_r.
+  intro x. rewrite* Multitype.union_empty_r.
+Qed.
+
+
+
+Lemma union_comm :
+  ∀ Γ₁ Γ₂, eq_ctx (Γ₁ ⊎c Γ₂) (Γ₂ ⊎c Γ₁).
+Proof.
+  Hint Resolve Multitype.union_comm : core.
+  intros [s₁ f₁] [s₂ f₂]; simpls*; splits*;
+  apply* union_comm.
+Qed.
+
+Lemma union_assoc :
+  ∀ Γ₁ Γ₂ Γ₃, eq_ctx ((Γ₁ ⊎c Γ₂) ⊎c Γ₃) (Γ₁ ⊎c (Γ₂ ⊎c Γ₃)).
+Proof.
+  Hint Resolve Multitype.union_assoc : core.
+  intros [s₁ f₁] [s₂ f₂] [s₃ f₃]; simpls*; splits*.
+  rewrite* union_assoc.
+Qed.
+
+
+Definition ok (Γ : ctx) : Prop := 
+  let (s, f) := Γ in 
+  ∀ x, x \in s <-> f x ≠ {{nil}}.
+
+
+Lemma ok_empty :
+  ok empty.
+Proof.
+  unfold empty. simpls.
+  intros; split; intro H_contra; exfalso.
+  applys* in_empty_inv. contradiction.
+Qed.
+Hint Resolve ok_empty : core.
+
+
+Lemma ok_add : 
+  ∀ (Γ : ctx) (x : var) (M : multitype),
+    ok Γ -> 
+    ok (add Γ x M).
+Proof.
+  introv Hok.
+  destruct Γ; simpls.
+  unfold add.
+  case_if*.
+  simpls.
+  split.
+  - intro H_in.
+    case_if; substs*.
+    + destruct (m x).
+      * rewrites* Multitype.union_empty_r.
+      * inductions M; autos*.
+        intro H_contra. inversion H_contra.
+    + specialize Hok with x0 as [H_in_nnil _].
+      rewrite in_union in H_in; destruct H_in; autos*.
+      rewrite in_singleton in H. autos*.
+  - case_if*; intro. substs*.
+    + rewrite in_union. right. rewrite* in_singleton.
+    + specialize Hok with x0 as [_ H_nnil_in].   
+      rewrite in_union. left*.
+Qed.
+
+Lemma nnil_union : 
+  ∀ mt1 mt2, 
+  mt1 ≠ {{ nil }} \/ mt2 ≠ {{ nil }} <->
+  mt1 ⊎ mt2 ≠ {{nil}}.
+Proof.
+  split.
+  - introv [Hmt1_nnil | Hmt2_nnil]; inductions mt1; autos*;
+    intro H_contra; inversion H_contra.
+  - intros H_nnil.
+    destruct mt1; simpls*.
+    left; intro H_contra; inversion H_contra.
+Qed.
+Lemma ok_union :
+  ∀ (Γ₁ Γ₂ : ctx),
+  ok Γ₁ -> ok Γ₂ ->
+  ok Γ₁ ⊎c Γ₂.
+Proof.
+  intros [s₁ f₁] [s₂ f₂] Hok1 Hok2.
+  intro x.
+  unfold ok in *.
+  specialize Hok1 with x as [H_in_nnil₁ H_nnil_in₁].
+  specialize Hok2 with x as [H_in_nnil₂ H_nnil_in₂].
+  split.
+  - intro H_in.
+    rewrite in_union in H_in.
+    destruct H_in as [H_in | H_in];
+    applys* nnil_union.
+  - intro. apply nnil_union in H as [H_f₁_x | H_f₂_x];
+    rewrite* in_union.
+Qed.
+
+Lemma ok_eq : 
+  ∀ Γ₁ Γ₂, 
+  eq_ctx Γ₁ Γ₂ ->
+  ok Γ₁ ->
+  ok Γ₂.
+Proof.
+  intros [s₁ f₁] [s₂ f₂] [H_eq_dom H_eq_f] Hok; simpls*.
+  intro x.
+  specialize Hok with x as [H_in_nnil H_nnil_in].
+  specialize H_eq_f with x; substs; split.
+  - intros H_in H_contra.
+    rewrite H_contra in *.
+    apply Multitype.eq_empty_is_empty in H_eq_f. autos*.
+  - intro H_nnil.
+    apply H_nnil_in.   
+    intro H_contra. rewrite H_contra in *.
+    apply Multitype.eq_sym in H_eq_f.
+    apply Multitype.eq_empty_is_empty in H_eq_f. autos*.
+Qed.
+
+Definition dom (Γ₁ : ctx) : vars := fst Γ₁.
+
+Lemma dom_add : 
+  ∀ Γ x mt,
+  mt ≠ {{nil}} ->
+  dom (add Γ x mt) = \{x} \u (dom Γ).
+Proof.
+  intros.
+  destruct Γ eqn:HeqΓ.
+  destruct (add (v, m) x mt) eqn:HeqAdd.
+  simpl.
+  unfold add in *.
+  case_if*.
+  inverts HeqAdd.
+  rewrite* LibFset.union_comm.
+Qed.
+
+Lemma dom_union :
+  ∀ Γ₁ Γ₂,
+  dom (Γ₁ ⊎c Γ₂) = (dom Γ₁) \u (dom Γ₂).
+Proof.
+  intros [s₁ f₁] [s₂ f₂].
+  simpls*.
+Qed.
+  
+
+
+Hint Resolve 
+  eq_refl eq_sym eq_trans 
+  union_empty_l union_empty_r
+  union_comm union_assoc
+  ok_empty ok_add nnil_union ok_union ok_eq 
+  dom_add dom_union 
+: core.
+Hint Unfold ok eq_ctx empty union_ctx dom : core.
