theories/Tactics.v
@@ -1,19 +1,73 @@
+From TLC Require Import LibFset LibTactics.
 
-Ltac absurd := 
-  let H := fresh in
-  intro H; inversion H; fail.
+Lemma split_subset :
+  forall (T : Type) (A B C : fset T),
+  A \u B \c C -> 
+  A \c C /\ B \c C.
+Proof.
+  intros.
+  split;
+  intros x Hin; unfold "\c" in H;
+  apply H; rewrite in_union; autos.
+Qed.
 
-Ltac myauto t := 
-               (absurd; fail) 
-            || (exfalso; eauto; fail)
-            || (t; fail)
-            || eauto.
-
-Tactic Notation "'myauto'" := myauto idtac.
-
-
-Ltac split_and := 
+Ltac split_and_or := 
   match goal with 
-  | [ |- _ /\ _ ] => split
-  | [H : _ /\ _ |- _] => destruct H
+  | [ |- _ /\ _] => split
+  | [ |- _ <-> _] => split
+  | [ H : _ /\ _ |- _] => 
+      let H1 := fresh H in
+      let H2 := fresh H in
+      destruct H as [H1 H2]
+  | [ H : _ <-> _ |- _] => 
+      let H1 := fresh H in
+      let H2 := fresh H in
+      destruct H as [H1 H2]
+  | [ H : _ \/ _ |- _] => 
+      destruct H as [H | H]
   end.
+
+Ltac simpl_unions := 
+  match goal with 
+  | [  |- context[\{} \u _] ] => rewrite LibFset.union_empty_l
+  | [  |- context[_ \u \{}] ] => rewrite LibFset.union_empty_r
+  | [ H : context[\{} \u _] |- _] => rewrite LibFset.union_empty_l in H
+  | [ H : context[_ \u \{}] |- _] => rewrite LibFset.union_empty_r in H
+  | [ H : context[_ \in \{}] |- _ ] => rewrite in_empty in H; contradiction
+  | [ H : context[_ \in \{ _ }] |- _ ] => rewrite in_singleton in H
+  | [  |- context[_ \in \{ _ }]] => rewrite in_singleton
+  | [  |- context[_ \in _ \u _]] => rewrite in_union
+  | [ H : context[_ \in _ \u _] |- _] => rewrite in_union in H
+  | [ H : context[_ \notin \{ _ }] |- _] => rewrite notin_singleton in H
+  | [ H : context[_ \notin _ \u _] |- _] => rewrite notin_union in H
+  | [ |- context[_ \notin \{ _ }]] => rewrite notin_singleton
+  | [ |- context[_ \notin _ \u _]] => rewrite notin_union
+  | [ H : context[_ \notin _ \u _] |- _] => rewrite notin_union in H
+  | [ H : _ \u _ \c _ |- _] => apply split_subset in H
+  | [ |- context[(_ \u _) \- _]] => rewrite union_remove
+  | [ H : context[(_ \u _) \- _] |- _] => rewrite union_remove in H
+  | [ H : context[_ \in _ \- _] |- _] => rewrite in_remove in H
+  | [ |- context[_ \in _ \- _] ] => rewrite in_remove
+  end.
+
+Ltac split_and_or_max := repeat split_and_or.
+
+Ltac use_equivalences := idtac.
+
+Ltac absurd := let H := fresh in intro H; inverts H; fail.
+
+Ltac reduce_max := repeat (simpl_unions || split_and_or).
+
+
+Lemma jmeq_to_eq :
+  forall A (v1 v2 : fset A), 
+  v1 = v2 -> JMeq.JMeq v1 v2.
+Proof.
+  intros; substs*.
+Qed.
+
+Ltac solve_set_equality :=
+  try apply jmeq_to_eq;
+  let x := fresh "x" in 
+  let Hin := fresh "Hin" x in 
+  apply fset_extens; intros x Hin; reduce_max; autos.
